<?xml version="1.0"?>
<rdf:RDF xmlns="http://www.semanticweb.org/shawr/ontologies/2022/10/RyanShaw_B00634437_CW1#"
     xml:base="http://www.semanticweb.org/shawr/ontologies/2022/10/RyanShaw_B00634437_CW1"
     xmlns:owl="http://www.w3.org/2002/07/owl#"
     xmlns:rdf="http://www.w3.org/1999/02/22-rdf-syntax-ns#"
     xmlns:xml="http://www.w3.org/XML/1998/namespace"
     xmlns:xsd="http://www.w3.org/2001/XMLSchema#"
     xmlns:rdfs="http://www.w3.org/2000/01/rdf-schema#">
    <owl:Ontology rdf:about="http://www.semanticweb.org/shawr/ontologies/2022/10/RyanShaw_B00634437_CW1">
        <rdfs:comment>An ontology for the 2019 general election results in Belfast constituencies domain.</rdfs:comment>
    </owl:Ontology>
    


    <!-- 
    ///////////////////////////////////////////////////////////////////////////////////////
    //
    // Object Properties
    //
    ///////////////////////////////////////////////////////////////////////////////////////
     -->

    


    <!-- http://www.semanticweb.org/shawr/ontologies/2022/10/RyanShaw_B00634437_CW1#hasAlignment -->

    <owl:ObjectProperty rdf:about="http://www.semanticweb.org/shawr/ontologies/2022/10/RyanShaw_B00634437_CW1#hasAlignment">
        <owl:inverseOf rdf:resource="http://www.semanticweb.org/shawr/ontologies/2022/10/RyanShaw_B00634437_CW1#isAlignmentFor"/>
        <rdfs:domain rdf:resource="http://www.semanticweb.org/shawr/ontologies/2022/10/RyanShaw_B00634437_CW1#Party"/>
        <rdfs:range rdf:resource="http://www.semanticweb.org/shawr/ontologies/2022/10/RyanShaw_B00634437_CW1#PoliticalAlignment"/>
        <rdfs:comment>The hasAlignment property represents the relationship between the Party class and the PoliticalAlignment class.</rdfs:comment>
    </owl:ObjectProperty>
    


    <!-- http://www.semanticweb.org/shawr/ontologies/2022/10/RyanShaw_B00634437_CW1#hasConstituency -->

    <owl:ObjectProperty rdf:about="http://www.semanticweb.org/shawr/ontologies/2022/10/RyanShaw_B00634437_CW1#hasConstituency">
        <owl:inverseOf rdf:resource="http://www.semanticweb.org/shawr/ontologies/2022/10/RyanShaw_B00634437_CW1#isConstituencyFor"/>
        <rdfs:domain rdf:resource="http://www.semanticweb.org/shawr/ontologies/2022/10/RyanShaw_B00634437_CW1#Candidate"/>
        <rdfs:range rdf:resource="http://www.semanticweb.org/shawr/ontologies/2022/10/RyanShaw_B00634437_CW1#Constituency"/>
        <rdfs:comment>The hasConstituency property represents the relationship between the Candidate class and the Constituency class.</rdfs:comment>
    </owl:ObjectProperty>
    


    <!-- http://www.semanticweb.org/shawr/ontologies/2022/10/RyanShaw_B00634437_CW1#hasElectedParty -->

    <owl:ObjectProperty rdf:about="http://www.semanticweb.org/shawr/ontologies/2022/10/RyanShaw_B00634437_CW1#hasElectedParty">
        <owl:inverseOf rdf:resource="http://www.semanticweb.org/shawr/ontologies/2022/10/RyanShaw_B00634437_CW1#isElectedPartyFor"/>
        <rdfs:domain rdf:resource="http://www.semanticweb.org/shawr/ontologies/2022/10/RyanShaw_B00634437_CW1#Constituency"/>
        <rdfs:range rdf:resource="http://www.semanticweb.org/shawr/ontologies/2022/10/RyanShaw_B00634437_CW1#ElectedParty"/>
        <rdfs:comment>The hasElectedParty property represents the relationship between the Constituency class and the Party class.</rdfs:comment>
    </owl:ObjectProperty>
    


    <!-- http://www.semanticweb.org/shawr/ontologies/2022/10/RyanShaw_B00634437_CW1#hasLessVotesThan -->

    <owl:ObjectProperty rdf:about="http://www.semanticweb.org/shawr/ontologies/2022/10/RyanShaw_B00634437_CW1#hasLessVotesThan">
        <owl:inverseOf rdf:resource="http://www.semanticweb.org/shawr/ontologies/2022/10/RyanShaw_B00634437_CW1#hasMoreVotesThan"/>
        <rdfs:comment>The hasMoreVotesThan property represents the inverse relationship between the individuals in the Candidate class.</rdfs:comment>
    </owl:ObjectProperty>
    


    <!-- http://www.semanticweb.org/shawr/ontologies/2022/10/RyanShaw_B00634437_CW1#hasMoreVotesThan -->

    <owl:ObjectProperty rdf:about="http://www.semanticweb.org/shawr/ontologies/2022/10/RyanShaw_B00634437_CW1#hasMoreVotesThan">
        <rdfs:domain rdf:resource="http://www.semanticweb.org/shawr/ontologies/2022/10/RyanShaw_B00634437_CW1#Candidate"/>
        <rdfs:range rdf:resource="http://www.semanticweb.org/shawr/ontologies/2022/10/RyanShaw_B00634437_CW1#Candidate"/>
        <rdfs:comment>The hasMoreVotesThan property represents the relationship between the individuals in the Candidate class.</rdfs:comment>
    </owl:ObjectProperty>
    


    <!-- http://www.semanticweb.org/shawr/ontologies/2022/10/RyanShaw_B00634437_CW1#hasParty -->

    <owl:ObjectProperty rdf:about="http://www.semanticweb.org/shawr/ontologies/2022/10/RyanShaw_B00634437_CW1#hasParty">
        <owl:inverseOf rdf:resource="http://www.semanticweb.org/shawr/ontologies/2022/10/RyanShaw_B00634437_CW1#isPartyFor"/>
        <rdfs:domain rdf:resource="http://www.semanticweb.org/shawr/ontologies/2022/10/RyanShaw_B00634437_CW1#Candidate"/>
        <rdfs:range rdf:resource="http://www.semanticweb.org/shawr/ontologies/2022/10/RyanShaw_B00634437_CW1#Party"/>
        <rdfs:comment>The hasParty property represents the relationship between the Candidate class and the Party class.</rdfs:comment>
    </owl:ObjectProperty>
    


    <!-- http://www.semanticweb.org/shawr/ontologies/2022/10/RyanShaw_B00634437_CW1#isAlignmentFor -->

    <owl:ObjectProperty rdf:about="http://www.semanticweb.org/shawr/ontologies/2022/10/RyanShaw_B00634437_CW1#isAlignmentFor">
        <rdfs:comment>The isAlignmentFor property represents the inverse relationship between the Party class and the PoliticalAlignment class.</rdfs:comment>
    </owl:ObjectProperty>
    


    <!-- http://www.semanticweb.org/shawr/ontologies/2022/10/RyanShaw_B00634437_CW1#isConstituencyFor -->

    <owl:ObjectProperty rdf:about="http://www.semanticweb.org/shawr/ontologies/2022/10/RyanShaw_B00634437_CW1#isConstituencyFor">
        <rdfs:comment>The isConstituencyFor property represents the inverse relationship between the Candidate class and the Constituency class.</rdfs:comment>
    </owl:ObjectProperty>
    


    <!-- http://www.semanticweb.org/shawr/ontologies/2022/10/RyanShaw_B00634437_CW1#isElectedPartyFor -->

    <owl:ObjectProperty rdf:about="http://www.semanticweb.org/shawr/ontologies/2022/10/RyanShaw_B00634437_CW1#isElectedPartyFor">
        <rdfs:comment>The isElectedPartyFor property represents the inverse relationship between the Constituency class and the Party class.</rdfs:comment>
    </owl:ObjectProperty>
    


    <!-- http://www.semanticweb.org/shawr/ontologies/2022/10/RyanShaw_B00634437_CW1#isPartyFor -->

    <owl:ObjectProperty rdf:about="http://www.semanticweb.org/shawr/ontologies/2022/10/RyanShaw_B00634437_CW1#isPartyFor">
        <rdfs:comment>The hasParty property represents the inverse relationship between the Candidate class and the Party class.</rdfs:comment>
    </owl:ObjectProperty>
    


    <!-- 
    ///////////////////////////////////////////////////////////////////////////////////////
    //
    // Data properties
    //
    ///////////////////////////////////////////////////////////////////////////////////////
     -->

    


    <!-- http://www.semanticweb.org/shawr/ontologies/2022/10/RyanShaw_B00634437_CW1#hasElectorate -->

    <owl:DatatypeProperty rdf:about="http://www.semanticweb.org/shawr/ontologies/2022/10/RyanShaw_B00634437_CW1#hasElectorate">
        <rdf:type rdf:resource="http://www.w3.org/2002/07/owl#FunctionalProperty"/>
        <rdfs:domain>
            <owl:Restriction>
                <owl:onProperty rdf:resource="http://www.semanticweb.org/shawr/ontologies/2022/10/RyanShaw_B00634437_CW1#hasElectorate"/>
                <owl:someValuesFrom rdf:resource="http://www.w3.org/2001/XMLSchema#integer"/>
            </owl:Restriction>
        </rdfs:domain>
        <rdfs:comment>The hasElectorate property represents the number of eligible voters in a constituency.</rdfs:comment>
    </owl:DatatypeProperty>
    


    <!-- http://www.semanticweb.org/shawr/ontologies/2022/10/RyanShaw_B00634437_CW1#hasMajority -->

    <owl:DatatypeProperty rdf:about="http://www.semanticweb.org/shawr/ontologies/2022/10/RyanShaw_B00634437_CW1#hasMajority">
        <rdf:type rdf:resource="http://www.w3.org/2002/07/owl#FunctionalProperty"/>
        <rdfs:domain>
            <owl:Restriction>
                <owl:onProperty rdf:resource="http://www.semanticweb.org/shawr/ontologies/2022/10/RyanShaw_B00634437_CW1#hasMajority"/>
                <owl:someValuesFrom rdf:resource="http://www.w3.org/2001/XMLSchema#integer"/>
            </owl:Restriction>
        </rdfs:domain>
        <rdfs:comment>The hasMajority property represents the majority held by a party in a constituency.</rdfs:comment>
    </owl:DatatypeProperty>
    


    <!-- http://www.semanticweb.org/shawr/ontologies/2022/10/RyanShaw_B00634437_CW1#hasOutcomeStatus -->

    <owl:DatatypeProperty rdf:about="http://www.semanticweb.org/shawr/ontologies/2022/10/RyanShaw_B00634437_CW1#hasOutcomeStatus">
        <rdf:type rdf:resource="http://www.w3.org/2002/07/owl#FunctionalProperty"/>
        <rdfs:domain>
            <owl:Restriction>
                <owl:onProperty rdf:resource="http://www.semanticweb.org/shawr/ontologies/2022/10/RyanShaw_B00634437_CW1#hasOutcomeStatus"/>
                <owl:someValuesFrom rdf:resource="http://www.w3.org/2001/XMLSchema#string"/>
            </owl:Restriction>
        </rdfs:domain>
        <rdfs:comment>The hasOutcomeStatus property represents whether a constituency was held or gained by a party.</rdfs:comment>
    </owl:DatatypeProperty>
    


    <!-- http://www.semanticweb.org/shawr/ontologies/2022/10/RyanShaw_B00634437_CW1#hasPercentageChangeInVote -->

    <owl:DatatypeProperty rdf:about="http://www.semanticweb.org/shawr/ontologies/2022/10/RyanShaw_B00634437_CW1#hasPercentageChangeInVote">
        <rdf:type rdf:resource="http://www.w3.org/2002/07/owl#FunctionalProperty"/>
        <rdfs:domain>
            <owl:Restriction>
                <owl:onProperty rdf:resource="http://www.semanticweb.org/shawr/ontologies/2022/10/RyanShaw_B00634437_CW1#hasPercentageChangeInVote"/>
                <owl:qualifiedCardinality rdf:datatype="http://www.w3.org/2001/XMLSchema#nonNegativeInteger">1</owl:qualifiedCardinality>
                <owl:onDataRange rdf:resource="http://www.w3.org/2001/XMLSchema#decimal"/>
            </owl:Restriction>
        </rdfs:domain>
        <rdfs:comment>The hasPercentageChangeInVote property represents the % change in the number of votes gained by a candidate in the 2019 general election when compared to the previous election.</rdfs:comment>
    </owl:DatatypeProperty>
    


    <!-- http://www.semanticweb.org/shawr/ontologies/2022/10/RyanShaw_B00634437_CW1#hasPercentageShareOfVote -->

    <owl:DatatypeProperty rdf:about="http://www.semanticweb.org/shawr/ontologies/2022/10/RyanShaw_B00634437_CW1#hasPercentageShareOfVote">
        <rdf:type rdf:resource="http://www.w3.org/2002/07/owl#FunctionalProperty"/>
        <rdfs:domain>
            <owl:Restriction>
                <owl:onProperty rdf:resource="http://www.semanticweb.org/shawr/ontologies/2022/10/RyanShaw_B00634437_CW1#hasPercentageShareOfVote"/>
                <owl:qualifiedCardinality rdf:datatype="http://www.w3.org/2001/XMLSchema#nonNegativeInteger">1</owl:qualifiedCardinality>
                <owl:onDataRange rdf:resource="http://www.w3.org/2001/XMLSchema#decimal"/>
            </owl:Restriction>
        </rdfs:domain>
        <rdfs:comment>The hasPercentageShareOfVote property represents the % share of the total number of votes gained by a candidate in the 2019 general election when compared to the previous election.</rdfs:comment>
    </owl:DatatypeProperty>
    


    <!-- http://www.semanticweb.org/shawr/ontologies/2022/10/RyanShaw_B00634437_CW1#hasTotalAveragePercentageChangeOfVote -->

    <owl:DatatypeProperty rdf:about="http://www.semanticweb.org/shawr/ontologies/2022/10/RyanShaw_B00634437_CW1#hasTotalAveragePercentageChangeOfVote">
        <rdf:type rdf:resource="http://www.w3.org/2002/07/owl#FunctionalProperty"/>
        <rdfs:domain>
            <owl:Restriction>
                <owl:onProperty rdf:resource="http://www.semanticweb.org/shawr/ontologies/2022/10/RyanShaw_B00634437_CW1#hasTotalAveragePercentageChangeOfVote"/>
                <owl:someValuesFrom rdf:resource="http://www.w3.org/2001/XMLSchema#decimal"/>
            </owl:Restriction>
        </rdfs:domain>
        <rdfs:comment>The hasTotalAveragePercentageChangeOfVote property represents the average % change of votes over all belfast constituencies gained by a party in the 2019 general election when compared to the previous election.</rdfs:comment>
    </owl:DatatypeProperty>
    


    <!-- http://www.semanticweb.org/shawr/ontologies/2022/10/RyanShaw_B00634437_CW1#hasTotalChangeInSeats -->

    <owl:DatatypeProperty rdf:about="http://www.semanticweb.org/shawr/ontologies/2022/10/RyanShaw_B00634437_CW1#hasTotalChangeInSeats">
        <rdf:type rdf:resource="http://www.w3.org/2002/07/owl#FunctionalProperty"/>
        <rdfs:domain>
            <owl:Restriction>
                <owl:onProperty rdf:resource="http://www.semanticweb.org/shawr/ontologies/2022/10/RyanShaw_B00634437_CW1#hasTotalChangeInSeats"/>
                <owl:someValuesFrom rdf:resource="http://www.w3.org/2001/XMLSchema#integer"/>
            </owl:Restriction>
        </rdfs:domain>
        <rdfs:comment>The hasTotalChangeInSeats property represents the change of seats gained by a party in the 2019 general election when compared to the previous election.</rdfs:comment>
    </owl:DatatypeProperty>
    


    <!-- http://www.semanticweb.org/shawr/ontologies/2022/10/RyanShaw_B00634437_CW1#hasTotalNumberOfCandidates -->

    <owl:DatatypeProperty rdf:about="http://www.semanticweb.org/shawr/ontologies/2022/10/RyanShaw_B00634437_CW1#hasTotalNumberOfCandidates">
        <rdf:type rdf:resource="http://www.w3.org/2002/07/owl#FunctionalProperty"/>
        <rdfs:domain>
            <owl:Restriction>
                <owl:onProperty rdf:resource="http://www.semanticweb.org/shawr/ontologies/2022/10/RyanShaw_B00634437_CW1#hasTotalNumberOfCandidates"/>
                <owl:someValuesFrom rdf:resource="http://www.w3.org/2001/XMLSchema#integer"/>
            </owl:Restriction>
        </rdfs:domain>
        <rdfs:comment>The hasTotalNumberOfCandidates property represents the total number of candidates a party had standing in the 2019 general election.</rdfs:comment>
    </owl:DatatypeProperty>
    


    <!-- http://www.semanticweb.org/shawr/ontologies/2022/10/RyanShaw_B00634437_CW1#hasTotalPercentageCandidateSuccessRate -->

    <owl:DatatypeProperty rdf:about="http://www.semanticweb.org/shawr/ontologies/2022/10/RyanShaw_B00634437_CW1#hasTotalPercentageCandidateSuccessRate">
        <rdf:type rdf:resource="http://www.w3.org/2002/07/owl#FunctionalProperty"/>
        <rdfs:domain>
            <owl:Restriction>
                <owl:onProperty rdf:resource="http://www.semanticweb.org/shawr/ontologies/2022/10/RyanShaw_B00634437_CW1#hasTotalPercentageCandidateSuccessRate"/>
                <owl:someValuesFrom rdf:resource="http://www.w3.org/2001/XMLSchema#integer"/>
            </owl:Restriction>
        </rdfs:domain>
        <rdfs:comment>The hasTotalPercentageCandidateSuccessRate property represents the % of a parties standing candidates who are successfully elected in the 2019 general election.</rdfs:comment>
    </owl:DatatypeProperty>
    


    <!-- http://www.semanticweb.org/shawr/ontologies/2022/10/RyanShaw_B00634437_CW1#hasTotalPercentageChangeInVote -->

    <owl:DatatypeProperty rdf:about="http://www.semanticweb.org/shawr/ontologies/2022/10/RyanShaw_B00634437_CW1#hasTotalPercentageChangeInVote">
        <rdf:type rdf:resource="http://www.w3.org/2002/07/owl#FunctionalProperty"/>
        <rdfs:domain>
            <owl:Restriction>
                <owl:onProperty rdf:resource="http://www.semanticweb.org/shawr/ontologies/2022/10/RyanShaw_B00634437_CW1#hasTotalPercentageChangeInVote"/>
                <owl:someValuesFrom rdf:resource="http://www.w3.org/2001/XMLSchema#decimal"/>
            </owl:Restriction>
        </rdfs:domain>
        <rdfs:comment>The hasTotalPercentageChangeOfVote property represents the % change of votes gained by a party in the 2019 general election when compared to the previous election.</rdfs:comment>
    </owl:DatatypeProperty>
    


    <!-- http://www.semanticweb.org/shawr/ontologies/2022/10/RyanShaw_B00634437_CW1#hasTotalPercentageShareOfVote -->

    <owl:DatatypeProperty rdf:about="http://www.semanticweb.org/shawr/ontologies/2022/10/RyanShaw_B00634437_CW1#hasTotalPercentageShareOfVote">
        <rdf:type rdf:resource="http://www.w3.org/2002/07/owl#FunctionalProperty"/>
        <rdfs:domain>
            <owl:Restriction>
                <owl:onProperty rdf:resource="http://www.semanticweb.org/shawr/ontologies/2022/10/RyanShaw_B00634437_CW1#hasTotalPercentageShareOfVote"/>
                <owl:someValuesFrom rdf:resource="http://www.w3.org/2001/XMLSchema#decimal"/>
            </owl:Restriction>
        </rdfs:domain>
        <rdfs:comment>The hasTotalPercentageShareOfVote property represents the % share of votes gained by a party in the 2019 general election.</rdfs:comment>
    </owl:DatatypeProperty>
    


    <!-- http://www.semanticweb.org/shawr/ontologies/2022/10/RyanShaw_B00634437_CW1#hasTotalSeatsWon -->

    <owl:DatatypeProperty rdf:about="http://www.semanticweb.org/shawr/ontologies/2022/10/RyanShaw_B00634437_CW1#hasTotalSeatsWon">
        <rdf:type rdf:resource="http://www.w3.org/2002/07/owl#FunctionalProperty"/>
        <rdfs:domain>
            <owl:Restriction>
                <owl:onProperty rdf:resource="http://www.semanticweb.org/shawr/ontologies/2022/10/RyanShaw_B00634437_CW1#hasTotalChangeInSeats"/>
                <owl:someValuesFrom rdf:resource="http://www.w3.org/2001/XMLSchema#integer"/>
            </owl:Restriction>
        </rdfs:domain>
        <rdfs:comment>The hasTotalSetasWon property represents the total number of seats won by a party in the 2019 general election when compared to the previous election.</rdfs:comment>
    </owl:DatatypeProperty>
    


    <!-- http://www.semanticweb.org/shawr/ontologies/2022/10/RyanShaw_B00634437_CW1#hasTotalVoteCount -->

    <owl:DatatypeProperty rdf:about="http://www.semanticweb.org/shawr/ontologies/2022/10/RyanShaw_B00634437_CW1#hasTotalVoteCount">
        <rdf:type rdf:resource="http://www.w3.org/2002/07/owl#FunctionalProperty"/>
        <rdfs:domain>
            <owl:Restriction>
                <owl:onProperty rdf:resource="http://www.semanticweb.org/shawr/ontologies/2022/10/RyanShaw_B00634437_CW1#hasTotalVoteCount"/>
                <owl:someValuesFrom rdf:resource="http://www.w3.org/2001/XMLSchema#integer"/>
            </owl:Restriction>
        </rdfs:domain>
        <rdfs:comment>The hasTotalVoteCount property represents the total number of votes gained by a party in the 2019 general election when compared to the previous election.</rdfs:comment>
    </owl:DatatypeProperty>
    


    <!-- http://www.semanticweb.org/shawr/ontologies/2022/10/RyanShaw_B00634437_CW1#hasTurnout -->

    <owl:DatatypeProperty rdf:about="http://www.semanticweb.org/shawr/ontologies/2022/10/RyanShaw_B00634437_CW1#hasTurnout">
        <rdf:type rdf:resource="http://www.w3.org/2002/07/owl#FunctionalProperty"/>
        <rdfs:domain>
            <owl:Restriction>
                <owl:onProperty rdf:resource="http://www.semanticweb.org/shawr/ontologies/2022/10/RyanShaw_B00634437_CW1#hasTurnout"/>
                <owl:someValuesFrom rdf:resource="http://www.w3.org/2001/XMLSchema#decimal"/>
            </owl:Restriction>
        </rdfs:domain>
        <rdfs:comment>The hasTurnout property represents the turnout % in a constituency.</rdfs:comment>
    </owl:DatatypeProperty>
    


    <!-- http://www.semanticweb.org/shawr/ontologies/2022/10/RyanShaw_B00634437_CW1#hasVoteCount -->

    <owl:DatatypeProperty rdf:about="http://www.semanticweb.org/shawr/ontologies/2022/10/RyanShaw_B00634437_CW1#hasVoteCount">
        <rdf:type rdf:resource="http://www.w3.org/2002/07/owl#FunctionalProperty"/>
        <rdfs:domain>
            <owl:Restriction>
                <owl:onProperty rdf:resource="http://www.semanticweb.org/shawr/ontologies/2022/10/RyanShaw_B00634437_CW1#hasVoteCount"/>
                <owl:qualifiedCardinality rdf:datatype="http://www.w3.org/2001/XMLSchema#nonNegativeInteger">1</owl:qualifiedCardinality>
                <owl:onDataRange rdf:resource="http://www.w3.org/2001/XMLSchema#integer"/>
            </owl:Restriction>
        </rdfs:domain>
        <rdfs:comment>The hasVoteCount property represents thethe number of votes gained by a candidate in the 2019 general election.</rdfs:comment>
    </owl:DatatypeProperty>
    


    <!-- 
    ///////////////////////////////////////////////////////////////////////////////////////
    //
    // Classes
    //
    ///////////////////////////////////////////////////////////////////////////////////////
     -->

    


    <!-- http://www.semanticweb.org/shawr/ontologies/2022/10/RyanShaw_B00634437_CW1#AllianceCandidate -->

    <owl:Class rdf:about="http://www.semanticweb.org/shawr/ontologies/2022/10/RyanShaw_B00634437_CW1#AllianceCandidate">
        <owl:equivalentClass>
            <owl:Class>
                <owl:intersectionOf rdf:parseType="Collection">
                    <rdf:Description rdf:about="http://www.semanticweb.org/shawr/ontologies/2022/10/RyanShaw_B00634437_CW1#Candidate"/>
                    <owl:Restriction>
                        <owl:onProperty rdf:resource="http://www.semanticweb.org/shawr/ontologies/2022/10/RyanShaw_B00634437_CW1#hasParty"/>
                        <owl:hasValue rdf:resource="http://www.semanticweb.org/shawr/ontologies/2022/10/RyanShaw_B00634437_CW1#Alliance"/>
                    </owl:Restriction>
                </owl:intersectionOf>
            </owl:Class>
        </owl:equivalentClass>
        <rdfs:comment>The AllianceCandidate class represents the set of individuals who are candidates for the Alliance party in the 2019 general election.</rdfs:comment>
    </owl:Class>
    


    <!-- http://www.semanticweb.org/shawr/ontologies/2022/10/RyanShaw_B00634437_CW1#AontuCandidate -->

    <owl:Class rdf:about="http://www.semanticweb.org/shawr/ontologies/2022/10/RyanShaw_B00634437_CW1#AontuCandidate">
        <owl:equivalentClass>
            <owl:Class>
                <owl:intersectionOf rdf:parseType="Collection">
                    <rdf:Description rdf:about="http://www.semanticweb.org/shawr/ontologies/2022/10/RyanShaw_B00634437_CW1#Candidate"/>
                    <owl:Restriction>
                        <owl:onProperty rdf:resource="http://www.semanticweb.org/shawr/ontologies/2022/10/RyanShaw_B00634437_CW1#hasParty"/>
                        <owl:hasValue rdf:resource="http://www.semanticweb.org/shawr/ontologies/2022/10/RyanShaw_B00634437_CW1#Aontu"/>
                    </owl:Restriction>
                </owl:intersectionOf>
            </owl:Class>
        </owl:equivalentClass>
        <rdfs:comment>The AontuCandidate class represents the set of individuals who are candidates for the Aonut party in the 2019 general election.</rdfs:comment>
    </owl:Class>
    


    <!-- http://www.semanticweb.org/shawr/ontologies/2022/10/RyanShaw_B00634437_CW1#BelfastEastCandidate -->

    <owl:Class rdf:about="http://www.semanticweb.org/shawr/ontologies/2022/10/RyanShaw_B00634437_CW1#BelfastEastCandidate">
        <owl:equivalentClass>
            <owl:Class>
                <owl:intersectionOf rdf:parseType="Collection">
                    <rdf:Description rdf:about="http://www.semanticweb.org/shawr/ontologies/2022/10/RyanShaw_B00634437_CW1#Candidate"/>
                    <owl:Restriction>
                        <owl:onProperty rdf:resource="http://www.semanticweb.org/shawr/ontologies/2022/10/RyanShaw_B00634437_CW1#hasConstituency"/>
                        <owl:hasValue rdf:resource="http://www.semanticweb.org/shawr/ontologies/2022/10/RyanShaw_B00634437_CW1#BelfastEast"/>
                    </owl:Restriction>
                </owl:intersectionOf>
            </owl:Class>
        </owl:equivalentClass>
        <rdfs:comment>The BelfastEastCandidate class represents the set of individuals who are candidates for the BelfastEast constituency in the 2019 general election.</rdfs:comment>
    </owl:Class>
    


    <!-- http://www.semanticweb.org/shawr/ontologies/2022/10/RyanShaw_B00634437_CW1#BelfastEastElectedCandidate -->

    <owl:Class rdf:about="http://www.semanticweb.org/shawr/ontologies/2022/10/RyanShaw_B00634437_CW1#BelfastEastElectedCandidate">
        <owl:equivalentClass>
            <owl:Class>
                <owl:intersectionOf rdf:parseType="Collection">
                    <rdf:Description rdf:about="http://www.semanticweb.org/shawr/ontologies/2022/10/RyanShaw_B00634437_CW1#Candidate"/>
                    <owl:Restriction>
                        <owl:onProperty rdf:resource="http://www.semanticweb.org/shawr/ontologies/2022/10/RyanShaw_B00634437_CW1#hasMoreVotesThan"/>
                        <owl:someValuesFrom rdf:resource="http://www.semanticweb.org/shawr/ontologies/2022/10/RyanShaw_B00634437_CW1#Candidate"/>
                    </owl:Restriction>
                    <owl:Restriction>
                        <owl:onProperty rdf:resource="http://www.semanticweb.org/shawr/ontologies/2022/10/RyanShaw_B00634437_CW1#hasConstituency"/>
                        <owl:hasValue rdf:resource="http://www.semanticweb.org/shawr/ontologies/2022/10/RyanShaw_B00634437_CW1#BelfastEast"/>
                    </owl:Restriction>
                </owl:intersectionOf>
            </owl:Class>
        </owl:equivalentClass>
        <rdfs:comment>The BelfastEastElectedCandidate class represents the set of individuals who are successfully elected candidates for the BelfastEast constituency in the 2019 general election.</rdfs:comment>
    </owl:Class>
    


    <!-- http://www.semanticweb.org/shawr/ontologies/2022/10/RyanShaw_B00634437_CW1#BelfastNorthCandidate -->

    <owl:Class rdf:about="http://www.semanticweb.org/shawr/ontologies/2022/10/RyanShaw_B00634437_CW1#BelfastNorthCandidate">
        <owl:equivalentClass>
            <owl:Class>
                <owl:intersectionOf rdf:parseType="Collection">
                    <rdf:Description rdf:about="http://www.semanticweb.org/shawr/ontologies/2022/10/RyanShaw_B00634437_CW1#Candidate"/>
                    <owl:Restriction>
                        <owl:onProperty rdf:resource="http://www.semanticweb.org/shawr/ontologies/2022/10/RyanShaw_B00634437_CW1#hasConstituency"/>
                        <owl:hasValue rdf:resource="http://www.semanticweb.org/shawr/ontologies/2022/10/RyanShaw_B00634437_CW1#BelfastNorth"/>
                    </owl:Restriction>
                </owl:intersectionOf>
            </owl:Class>
        </owl:equivalentClass>
        <rdfs:comment>The BelfastNorthCandidate class represents the set of individuals who are candidates for the BelfastNorth constituency in the 2019 general election.</rdfs:comment>
    </owl:Class>
    


    <!-- http://www.semanticweb.org/shawr/ontologies/2022/10/RyanShaw_B00634437_CW1#BelfastNorthElectedCandidate -->

    <owl:Class rdf:about="http://www.semanticweb.org/shawr/ontologies/2022/10/RyanShaw_B00634437_CW1#BelfastNorthElectedCandidate">
        <owl:equivalentClass>
            <owl:Class>
                <owl:intersectionOf rdf:parseType="Collection">
                    <rdf:Description rdf:about="http://www.semanticweb.org/shawr/ontologies/2022/10/RyanShaw_B00634437_CW1#Candidate"/>
                    <owl:Restriction>
                        <owl:onProperty rdf:resource="http://www.semanticweb.org/shawr/ontologies/2022/10/RyanShaw_B00634437_CW1#hasMoreVotesThan"/>
                        <owl:someValuesFrom rdf:resource="http://www.semanticweb.org/shawr/ontologies/2022/10/RyanShaw_B00634437_CW1#Candidate"/>
                    </owl:Restriction>
                    <owl:Restriction>
                        <owl:onProperty rdf:resource="http://www.semanticweb.org/shawr/ontologies/2022/10/RyanShaw_B00634437_CW1#hasConstituency"/>
                        <owl:hasValue rdf:resource="http://www.semanticweb.org/shawr/ontologies/2022/10/RyanShaw_B00634437_CW1#BelfastNorth"/>
                    </owl:Restriction>
                </owl:intersectionOf>
            </owl:Class>
        </owl:equivalentClass>
        <rdfs:comment>The BelfastNorthElectedCandidate class represents the set of individuals who are successfully elected candidates for the BelfastNorth constituency in the 2019 general election.</rdfs:comment>
    </owl:Class>
    


    <!-- http://www.semanticweb.org/shawr/ontologies/2022/10/RyanShaw_B00634437_CW1#BelfastSouthCandidate -->

    <owl:Class rdf:about="http://www.semanticweb.org/shawr/ontologies/2022/10/RyanShaw_B00634437_CW1#BelfastSouthCandidate">
        <owl:equivalentClass>
            <owl:Class>
                <owl:intersectionOf rdf:parseType="Collection">
                    <rdf:Description rdf:about="http://www.semanticweb.org/shawr/ontologies/2022/10/RyanShaw_B00634437_CW1#Candidate"/>
                    <owl:Restriction>
                        <owl:onProperty rdf:resource="http://www.semanticweb.org/shawr/ontologies/2022/10/RyanShaw_B00634437_CW1#hasConstituency"/>
                        <owl:hasValue rdf:resource="http://www.semanticweb.org/shawr/ontologies/2022/10/RyanShaw_B00634437_CW1#BelfastSouth"/>
                    </owl:Restriction>
                </owl:intersectionOf>
            </owl:Class>
        </owl:equivalentClass>
        <rdfs:comment>The BelfastSouthCandidate class represents the set of individuals who are candidates for the BelfastSouth constituency in the 2019 general election.</rdfs:comment>
    </owl:Class>
    


    <!-- http://www.semanticweb.org/shawr/ontologies/2022/10/RyanShaw_B00634437_CW1#BelfastSouthElectedCandidate -->

    <owl:Class rdf:about="http://www.semanticweb.org/shawr/ontologies/2022/10/RyanShaw_B00634437_CW1#BelfastSouthElectedCandidate">
        <owl:equivalentClass>
            <owl:Class>
                <owl:intersectionOf rdf:parseType="Collection">
                    <rdf:Description rdf:about="http://www.semanticweb.org/shawr/ontologies/2022/10/RyanShaw_B00634437_CW1#Candidate"/>
                    <owl:Restriction>
                        <owl:onProperty rdf:resource="http://www.semanticweb.org/shawr/ontologies/2022/10/RyanShaw_B00634437_CW1#hasMoreVotesThan"/>
                        <owl:someValuesFrom rdf:resource="http://www.semanticweb.org/shawr/ontologies/2022/10/RyanShaw_B00634437_CW1#Candidate"/>
                    </owl:Restriction>
                    <owl:Restriction>
                        <owl:onProperty rdf:resource="http://www.semanticweb.org/shawr/ontologies/2022/10/RyanShaw_B00634437_CW1#hasConstituency"/>
                        <owl:hasValue rdf:resource="http://www.semanticweb.org/shawr/ontologies/2022/10/RyanShaw_B00634437_CW1#BelfastSouth"/>
                    </owl:Restriction>
                </owl:intersectionOf>
            </owl:Class>
        </owl:equivalentClass>
        <rdfs:comment>The BelfastSouthElectedCandidate class represents the set of individuals who are successfully elected candidates for the BelfastSouth constituency in the 2019 general election.</rdfs:comment>
    </owl:Class>
    


    <!-- http://www.semanticweb.org/shawr/ontologies/2022/10/RyanShaw_B00634437_CW1#BelfastWestCandidate -->

    <owl:Class rdf:about="http://www.semanticweb.org/shawr/ontologies/2022/10/RyanShaw_B00634437_CW1#BelfastWestCandidate">
        <owl:equivalentClass>
            <owl:Class>
                <owl:intersectionOf rdf:parseType="Collection">
                    <rdf:Description rdf:about="http://www.semanticweb.org/shawr/ontologies/2022/10/RyanShaw_B00634437_CW1#Candidate"/>
                    <owl:Restriction>
                        <owl:onProperty rdf:resource="http://www.semanticweb.org/shawr/ontologies/2022/10/RyanShaw_B00634437_CW1#hasConstituency"/>
                        <owl:hasValue rdf:resource="http://www.semanticweb.org/shawr/ontologies/2022/10/RyanShaw_B00634437_CW1#BelfastWest"/>
                    </owl:Restriction>
                </owl:intersectionOf>
            </owl:Class>
        </owl:equivalentClass>
        <rdfs:comment>The BelfastWestCandidate class represents the set of individuals who are candidates for the BelfastWest constituency in the 2019 general election.</rdfs:comment>
    </owl:Class>
    


    <!-- http://www.semanticweb.org/shawr/ontologies/2022/10/RyanShaw_B00634437_CW1#BelfastWestElectedCandidate -->

    <owl:Class rdf:about="http://www.semanticweb.org/shawr/ontologies/2022/10/RyanShaw_B00634437_CW1#BelfastWestElectedCandidate">
        <owl:equivalentClass>
            <owl:Class>
                <owl:intersectionOf rdf:parseType="Collection">
                    <rdf:Description rdf:about="http://www.semanticweb.org/shawr/ontologies/2022/10/RyanShaw_B00634437_CW1#Candidate"/>
                    <owl:Restriction>
                        <owl:onProperty rdf:resource="http://www.semanticweb.org/shawr/ontologies/2022/10/RyanShaw_B00634437_CW1#hasMoreVotesThan"/>
                        <owl:someValuesFrom rdf:resource="http://www.semanticweb.org/shawr/ontologies/2022/10/RyanShaw_B00634437_CW1#Candidate"/>
                    </owl:Restriction>
                    <owl:Restriction>
                        <owl:onProperty rdf:resource="http://www.semanticweb.org/shawr/ontologies/2022/10/RyanShaw_B00634437_CW1#hasConstituency"/>
                        <owl:hasValue rdf:resource="http://www.semanticweb.org/shawr/ontologies/2022/10/RyanShaw_B00634437_CW1#BelfastWest"/>
                    </owl:Restriction>
                </owl:intersectionOf>
            </owl:Class>
        </owl:equivalentClass>
        <rdfs:comment>The BelfastWestElectedCandidate class represents the set of individuals who are successfully elected candidates for the BelfastWest constituency in the 2019 general election.</rdfs:comment>
    </owl:Class>
    


    <!-- http://www.semanticweb.org/shawr/ontologies/2022/10/RyanShaw_B00634437_CW1#Candidate -->

    <owl:Class rdf:about="http://www.semanticweb.org/shawr/ontologies/2022/10/RyanShaw_B00634437_CW1#Candidate">
        <rdfs:subClassOf>
            <owl:Restriction>
                <owl:onProperty rdf:resource="http://www.semanticweb.org/shawr/ontologies/2022/10/RyanShaw_B00634437_CW1#hasConstituency"/>
                <owl:qualifiedCardinality rdf:datatype="http://www.w3.org/2001/XMLSchema#nonNegativeInteger">1</owl:qualifiedCardinality>
                <owl:onClass rdf:resource="http://www.semanticweb.org/shawr/ontologies/2022/10/RyanShaw_B00634437_CW1#Constituency"/>
            </owl:Restriction>
        </rdfs:subClassOf>
        <rdfs:subClassOf>
            <owl:Restriction>
                <owl:onProperty rdf:resource="http://www.semanticweb.org/shawr/ontologies/2022/10/RyanShaw_B00634437_CW1#hasParty"/>
                <owl:qualifiedCardinality rdf:datatype="http://www.w3.org/2001/XMLSchema#nonNegativeInteger">1</owl:qualifiedCardinality>
                <owl:onClass rdf:resource="http://www.semanticweb.org/shawr/ontologies/2022/10/RyanShaw_B00634437_CW1#Party"/>
            </owl:Restriction>
        </rdfs:subClassOf>
        <rdfs:comment>The Candidate class represents the set of individuals who stood in Belfast constituencies in the 2019 general election.</rdfs:comment>
    </owl:Class>
    


    <!-- http://www.semanticweb.org/shawr/ontologies/2022/10/RyanShaw_B00634437_CW1#Constituency -->

    <owl:Class rdf:about="http://www.semanticweb.org/shawr/ontologies/2022/10/RyanShaw_B00634437_CW1#Constituency">
        <rdfs:comment>The Constituency class represents the set of individual Belfast constituencies in the 2019 general election.</rdfs:comment>
    </owl:Class>
    


    <!-- http://www.semanticweb.org/shawr/ontologies/2022/10/RyanShaw_B00634437_CW1#DUPCandidate -->

    <owl:Class rdf:about="http://www.semanticweb.org/shawr/ontologies/2022/10/RyanShaw_B00634437_CW1#DUPCandidate">
        <owl:equivalentClass>
            <owl:Class>
                <owl:intersectionOf rdf:parseType="Collection">
                    <rdf:Description rdf:about="http://www.semanticweb.org/shawr/ontologies/2022/10/RyanShaw_B00634437_CW1#Candidate"/>
                    <owl:Restriction>
                        <owl:onProperty rdf:resource="http://www.semanticweb.org/shawr/ontologies/2022/10/RyanShaw_B00634437_CW1#hasParty"/>
                        <owl:hasValue rdf:resource="http://www.semanticweb.org/shawr/ontologies/2022/10/RyanShaw_B00634437_CW1#DUP"/>
                    </owl:Restriction>
                </owl:intersectionOf>
            </owl:Class>
        </owl:equivalentClass>
        <rdfs:comment>The DUPCandidate class represents the set of individuals who are candidates for the DUP party in the 2019 general election.</rdfs:comment>
    </owl:Class>
    


    <!-- http://www.semanticweb.org/shawr/ontologies/2022/10/RyanShaw_B00634437_CW1#DUPConstituency -->

    <owl:Class rdf:about="http://www.semanticweb.org/shawr/ontologies/2022/10/RyanShaw_B00634437_CW1#DUPConstituency">
        <owl:equivalentClass>
            <owl:Class>
                <owl:intersectionOf rdf:parseType="Collection">
                    <rdf:Description rdf:about="http://www.semanticweb.org/shawr/ontologies/2022/10/RyanShaw_B00634437_CW1#Constituency"/>
                    <owl:Restriction>
                        <owl:onProperty rdf:resource="http://www.semanticweb.org/shawr/ontologies/2022/10/RyanShaw_B00634437_CW1#hasElectedParty"/>
                        <owl:hasValue rdf:resource="http://www.semanticweb.org/shawr/ontologies/2022/10/RyanShaw_B00634437_CW1#DUP"/>
                    </owl:Restriction>
                </owl:intersectionOf>
            </owl:Class>
        </owl:equivalentClass>
        <rdfs:comment>The DUPConstituency class represents the set of individual Belfast constituencies won by the DUP party in the 2019 general election.</rdfs:comment>
    </owl:Class>
    


    <!-- http://www.semanticweb.org/shawr/ontologies/2022/10/RyanShaw_B00634437_CW1#ElectedParty -->

    <owl:Class rdf:about="http://www.semanticweb.org/shawr/ontologies/2022/10/RyanShaw_B00634437_CW1#ElectedParty">
        <owl:equivalentClass>
            <owl:Class>
                <owl:intersectionOf rdf:parseType="Collection">
                    <rdf:Description rdf:about="http://www.semanticweb.org/shawr/ontologies/2022/10/RyanShaw_B00634437_CW1#Party"/>
                    <owl:Restriction>
                        <owl:onProperty rdf:resource="http://www.semanticweb.org/shawr/ontologies/2022/10/RyanShaw_B00634437_CW1#hasTotalSeatsWon"/>
                        <owl:someValuesFrom>
                            <rdfs:Datatype>
                                <owl:onDatatype rdf:resource="http://www.w3.org/2001/XMLSchema#decimal"/>
                                <owl:withRestrictions rdf:parseType="Collection">
                                    <rdf:Description>
                                        <xsd:minExclusive rdf:datatype="http://www.w3.org/2001/XMLSchema#decimal">0</xsd:minExclusive>
                                    </rdf:Description>
                                </owl:withRestrictions>
                            </rdfs:Datatype>
                        </owl:someValuesFrom>
                    </owl:Restriction>
                </owl:intersectionOf>
            </owl:Class>
        </owl:equivalentClass>
        <rdfs:comment>The Party class represents the set of individual parties who had candidates elected in Belfast constituencies in the the 2019 general election.</rdfs:comment>
    </owl:Class>
    


    <!-- http://www.semanticweb.org/shawr/ontologies/2022/10/RyanShaw_B00634437_CW1#GainedSeatsParty -->

    <owl:Class rdf:about="http://www.semanticweb.org/shawr/ontologies/2022/10/RyanShaw_B00634437_CW1#GainedSeatsParty">
        <owl:equivalentClass>
            <owl:Class>
                <owl:intersectionOf rdf:parseType="Collection">
                    <rdf:Description rdf:about="http://www.semanticweb.org/shawr/ontologies/2022/10/RyanShaw_B00634437_CW1#Party"/>
                    <owl:Restriction>
                        <owl:onProperty rdf:resource="http://www.semanticweb.org/shawr/ontologies/2022/10/RyanShaw_B00634437_CW1#hasTotalChangeInSeats"/>
                        <owl:someValuesFrom>
                            <rdfs:Datatype>
                                <owl:onDatatype rdf:resource="http://www.w3.org/2001/XMLSchema#integer"/>
                                <owl:withRestrictions rdf:parseType="Collection">
                                    <rdf:Description>
                                        <xsd:minExclusive rdf:datatype="http://www.w3.org/2001/XMLSchema#integer">0</xsd:minExclusive>
                                    </rdf:Description>
                                </owl:withRestrictions>
                            </rdfs:Datatype>
                        </owl:someValuesFrom>
                    </owl:Restriction>
                </owl:intersectionOf>
            </owl:Class>
        </owl:equivalentClass>
        <rdfs:comment>The GainedSeatsParty class represents the set of individual parties who gained seats in the the 2019 general election when compared to the previous election.</rdfs:comment>
    </owl:Class>
    


    <!-- http://www.semanticweb.org/shawr/ontologies/2022/10/RyanShaw_B00634437_CW1#GainedVotesCandidate -->

    <owl:Class rdf:about="http://www.semanticweb.org/shawr/ontologies/2022/10/RyanShaw_B00634437_CW1#GainedVotesCandidate">
        <owl:equivalentClass>
            <owl:Class>
                <owl:intersectionOf rdf:parseType="Collection">
                    <rdf:Description rdf:about="http://www.semanticweb.org/shawr/ontologies/2022/10/RyanShaw_B00634437_CW1#Candidate"/>
                    <owl:Restriction>
                        <owl:onProperty rdf:resource="http://www.semanticweb.org/shawr/ontologies/2022/10/RyanShaw_B00634437_CW1#hasPercentageChangeInVote"/>
                        <owl:someValuesFrom>
                            <rdfs:Datatype>
                                <owl:onDatatype rdf:resource="http://www.w3.org/2001/XMLSchema#decimal"/>
                                <owl:withRestrictions rdf:parseType="Collection">
                                    <rdf:Description>
                                        <xsd:minExclusive rdf:datatype="http://www.w3.org/2001/XMLSchema#decimal">0</xsd:minExclusive>
                                    </rdf:Description>
                                </owl:withRestrictions>
                            </rdfs:Datatype>
                        </owl:someValuesFrom>
                    </owl:Restriction>
                </owl:intersectionOf>
            </owl:Class>
        </owl:equivalentClass>
        <rdfs:comment>The GainedVotesCandidate class represents the set of individuals who had a increase in votes in the 2019 general election when compared to the previous election.</rdfs:comment>
    </owl:Class>
    


    <!-- http://www.semanticweb.org/shawr/ontologies/2022/10/RyanShaw_B00634437_CW1#GainedVotesParty -->

    <owl:Class rdf:about="http://www.semanticweb.org/shawr/ontologies/2022/10/RyanShaw_B00634437_CW1#GainedVotesParty">
        <owl:equivalentClass>
            <owl:Class>
                <owl:intersectionOf rdf:parseType="Collection">
                    <rdf:Description rdf:about="http://www.semanticweb.org/shawr/ontologies/2022/10/RyanShaw_B00634437_CW1#Party"/>
                    <owl:Restriction>
                        <owl:onProperty rdf:resource="http://www.semanticweb.org/shawr/ontologies/2022/10/RyanShaw_B00634437_CW1#hasTotalPercentageChangeInVote"/>
                        <owl:someValuesFrom>
                            <rdfs:Datatype>
                                <owl:onDatatype rdf:resource="http://www.w3.org/2001/XMLSchema#decimal"/>
                                <owl:withRestrictions rdf:parseType="Collection">
                                    <rdf:Description>
                                        <xsd:minExclusive rdf:datatype="http://www.w3.org/2001/XMLSchema#decimal">0</xsd:minExclusive>
                                    </rdf:Description>
                                </owl:withRestrictions>
                            </rdfs:Datatype>
                        </owl:someValuesFrom>
                    </owl:Restriction>
                </owl:intersectionOf>
            </owl:Class>
        </owl:equivalentClass>
        <rdfs:comment>The GainedVotesParty class represents the set of individual parties who gained votes in the the 2019 general election when compared to the previous election.</rdfs:comment>
    </owl:Class>
    


    <!-- http://www.semanticweb.org/shawr/ontologies/2022/10/RyanShaw_B00634437_CW1#LostSeatsParty -->

    <owl:Class rdf:about="http://www.semanticweb.org/shawr/ontologies/2022/10/RyanShaw_B00634437_CW1#LostSeatsParty">
        <owl:equivalentClass>
            <owl:Class>
                <owl:intersectionOf rdf:parseType="Collection">
                    <rdf:Description rdf:about="http://www.semanticweb.org/shawr/ontologies/2022/10/RyanShaw_B00634437_CW1#Party"/>
                    <owl:Restriction>
                        <owl:onProperty rdf:resource="http://www.semanticweb.org/shawr/ontologies/2022/10/RyanShaw_B00634437_CW1#hasTotalChangeInSeats"/>
                        <owl:someValuesFrom>
                            <rdfs:Datatype>
                                <owl:onDatatype rdf:resource="http://www.w3.org/2001/XMLSchema#integer"/>
                                <owl:withRestrictions rdf:parseType="Collection">
                                    <rdf:Description>
                                        <xsd:maxExclusive rdf:datatype="http://www.w3.org/2001/XMLSchema#integer">0</xsd:maxExclusive>
                                    </rdf:Description>
                                </owl:withRestrictions>
                            </rdfs:Datatype>
                        </owl:someValuesFrom>
                    </owl:Restriction>
                </owl:intersectionOf>
            </owl:Class>
        </owl:equivalentClass>
        <rdfs:comment>The LostSeatsParty class represents the set of individual parties who lost seats in the the 2019 general election when compared to the previous election.</rdfs:comment>
    </owl:Class>
    


    <!-- http://www.semanticweb.org/shawr/ontologies/2022/10/RyanShaw_B00634437_CW1#LostVotesCandidate -->

    <owl:Class rdf:about="http://www.semanticweb.org/shawr/ontologies/2022/10/RyanShaw_B00634437_CW1#LostVotesCandidate">
        <owl:equivalentClass>
            <owl:Class>
                <owl:intersectionOf rdf:parseType="Collection">
                    <rdf:Description rdf:about="http://www.semanticweb.org/shawr/ontologies/2022/10/RyanShaw_B00634437_CW1#Candidate"/>
                    <owl:Restriction>
                        <owl:onProperty rdf:resource="http://www.semanticweb.org/shawr/ontologies/2022/10/RyanShaw_B00634437_CW1#hasPercentageChangeInVote"/>
                        <owl:someValuesFrom>
                            <rdfs:Datatype>
                                <owl:onDatatype rdf:resource="http://www.w3.org/2001/XMLSchema#decimal"/>
                                <owl:withRestrictions rdf:parseType="Collection">
                                    <rdf:Description>
                                        <xsd:maxExclusive rdf:datatype="http://www.w3.org/2001/XMLSchema#decimal">0</xsd:maxExclusive>
                                    </rdf:Description>
                                </owl:withRestrictions>
                            </rdfs:Datatype>
                        </owl:someValuesFrom>
                    </owl:Restriction>
                </owl:intersectionOf>
            </owl:Class>
        </owl:equivalentClass>
        <rdfs:comment>The LostVotesCandidate class represents the set of individuals who had a decrease in votes in the 2019 general election when compared to the previous election.</rdfs:comment>
    </owl:Class>
    


    <!-- http://www.semanticweb.org/shawr/ontologies/2022/10/RyanShaw_B00634437_CW1#LostVotesParty -->

    <owl:Class rdf:about="http://www.semanticweb.org/shawr/ontologies/2022/10/RyanShaw_B00634437_CW1#LostVotesParty">
        <owl:equivalentClass>
            <owl:Class>
                <owl:intersectionOf rdf:parseType="Collection">
                    <rdf:Description rdf:about="http://www.semanticweb.org/shawr/ontologies/2022/10/RyanShaw_B00634437_CW1#Party"/>
                    <owl:Restriction>
                        <owl:onProperty rdf:resource="http://www.semanticweb.org/shawr/ontologies/2022/10/RyanShaw_B00634437_CW1#hasTotalPercentageChangeInVote"/>
                        <owl:someValuesFrom>
                            <rdfs:Datatype>
                                <owl:onDatatype rdf:resource="http://www.w3.org/2001/XMLSchema#decimal"/>
                                <owl:withRestrictions rdf:parseType="Collection">
                                    <rdf:Description>
                                        <xsd:maxExclusive rdf:datatype="http://www.w3.org/2001/XMLSchema#decimal">0</xsd:maxExclusive>
                                    </rdf:Description>
                                </owl:withRestrictions>
                            </rdfs:Datatype>
                        </owl:someValuesFrom>
                    </owl:Restriction>
                </owl:intersectionOf>
            </owl:Class>
        </owl:equivalentClass>
        <rdfs:comment>The LostVotesParty class represents the set of individual parties who lost votes in the the 2019 general election when compared to the previous election.</rdfs:comment>
    </owl:Class>
    


    <!-- http://www.semanticweb.org/shawr/ontologies/2022/10/RyanShaw_B00634437_CW1#NationalistCandidate -->

    <owl:Class rdf:about="http://www.semanticweb.org/shawr/ontologies/2022/10/RyanShaw_B00634437_CW1#NationalistCandidate">
        <owl:equivalentClass>
            <owl:Class>
                <owl:intersectionOf rdf:parseType="Collection">
                    <rdf:Description rdf:about="http://www.semanticweb.org/shawr/ontologies/2022/10/RyanShaw_B00634437_CW1#Candidate"/>
                    <owl:Restriction>
                        <owl:onProperty rdf:resource="http://www.semanticweb.org/shawr/ontologies/2022/10/RyanShaw_B00634437_CW1#hasParty"/>
                        <owl:someValuesFrom rdf:resource="http://www.semanticweb.org/shawr/ontologies/2022/10/RyanShaw_B00634437_CW1#NationalistParty"/>
                    </owl:Restriction>
                </owl:intersectionOf>
            </owl:Class>
        </owl:equivalentClass>
        <rdfs:comment>The NationalistCandidate class represents the set of individuals who are candidates for parties with Nationalist political alignment  in the 2019 general election.</rdfs:comment>
    </owl:Class>
    


    <!-- http://www.semanticweb.org/shawr/ontologies/2022/10/RyanShaw_B00634437_CW1#NationalistParty -->

    <owl:Class rdf:about="http://www.semanticweb.org/shawr/ontologies/2022/10/RyanShaw_B00634437_CW1#NationalistParty">
        <owl:equivalentClass>
            <owl:Class>
                <owl:intersectionOf rdf:parseType="Collection">
                    <rdf:Description rdf:about="http://www.semanticweb.org/shawr/ontologies/2022/10/RyanShaw_B00634437_CW1#Party"/>
                    <owl:Restriction>
                        <owl:onProperty rdf:resource="http://www.semanticweb.org/shawr/ontologies/2022/10/RyanShaw_B00634437_CW1#hasAlignment"/>
                        <owl:hasValue rdf:resource="http://www.semanticweb.org/shawr/ontologies/2022/10/RyanShaw_B00634437_CW1#Nationlist"/>
                    </owl:Restriction>
                </owl:intersectionOf>
            </owl:Class>
        </owl:equivalentClass>
        <rdfs:comment>The NationlistParty class represents the set of individual parties who had a Nationalist political alignment in the the 2019 general election.</rdfs:comment>
    </owl:Class>
    


    <!-- http://www.semanticweb.org/shawr/ontologies/2022/10/RyanShaw_B00634437_CW1#NationlistConstituency -->

    <owl:Class rdf:about="http://www.semanticweb.org/shawr/ontologies/2022/10/RyanShaw_B00634437_CW1#NationlistConstituency">
        <owl:equivalentClass>
            <owl:Class>
                <owl:intersectionOf rdf:parseType="Collection">
                    <rdf:Description rdf:about="http://www.semanticweb.org/shawr/ontologies/2022/10/RyanShaw_B00634437_CW1#Constituency"/>
                    <owl:Restriction>
                        <owl:onProperty rdf:resource="http://www.semanticweb.org/shawr/ontologies/2022/10/RyanShaw_B00634437_CW1#hasElectedParty"/>
                        <owl:someValuesFrom rdf:resource="http://www.semanticweb.org/shawr/ontologies/2022/10/RyanShaw_B00634437_CW1#NationalistParty"/>
                    </owl:Restriction>
                </owl:intersectionOf>
            </owl:Class>
        </owl:equivalentClass>
        <rdfs:comment>The NationalistConstituency class represents the set of individual Belfast constituencies won by parties with a Nationalist political alignment in the 2019 general election.</rdfs:comment>
    </owl:Class>
    


    <!-- http://www.semanticweb.org/shawr/ontologies/2022/10/RyanShaw_B00634437_CW1#NondesignateCandidate -->

    <owl:Class rdf:about="http://www.semanticweb.org/shawr/ontologies/2022/10/RyanShaw_B00634437_CW1#NondesignateCandidate">
        <owl:equivalentClass>
            <owl:Class>
                <owl:intersectionOf rdf:parseType="Collection">
                    <rdf:Description rdf:about="http://www.semanticweb.org/shawr/ontologies/2022/10/RyanShaw_B00634437_CW1#Candidate"/>
                    <owl:Restriction>
                        <owl:onProperty rdf:resource="http://www.semanticweb.org/shawr/ontologies/2022/10/RyanShaw_B00634437_CW1#hasParty"/>
                        <owl:someValuesFrom rdf:resource="http://www.semanticweb.org/shawr/ontologies/2022/10/RyanShaw_B00634437_CW1#NondesignateParty"/>
                    </owl:Restriction>
                </owl:intersectionOf>
            </owl:Class>
        </owl:equivalentClass>
        <rdfs:comment>The NondesignateCandidate class represents the set of individuals who are candidates for parties with Nondesignate political alignment  in the 2019 general election.</rdfs:comment>
    </owl:Class>
    


    <!-- http://www.semanticweb.org/shawr/ontologies/2022/10/RyanShaw_B00634437_CW1#NondesignateParty -->

    <owl:Class rdf:about="http://www.semanticweb.org/shawr/ontologies/2022/10/RyanShaw_B00634437_CW1#NondesignateParty">
        <owl:equivalentClass>
            <owl:Class>
                <owl:intersectionOf rdf:parseType="Collection">
                    <rdf:Description rdf:about="http://www.semanticweb.org/shawr/ontologies/2022/10/RyanShaw_B00634437_CW1#Party"/>
                    <owl:Restriction>
                        <owl:onProperty rdf:resource="http://www.semanticweb.org/shawr/ontologies/2022/10/RyanShaw_B00634437_CW1#hasAlignment"/>
                        <owl:hasValue rdf:resource="http://www.semanticweb.org/shawr/ontologies/2022/10/RyanShaw_B00634437_CW1#Nondesignate"/>
                    </owl:Restriction>
                </owl:intersectionOf>
            </owl:Class>
        </owl:equivalentClass>
        <rdfs:comment>The NondesignateParty class represents the set of individual parties who had a Nondesignate political alignment in the the 2019 general election.</rdfs:comment>
    </owl:Class>
    


    <!-- http://www.semanticweb.org/shawr/ontologies/2022/10/RyanShaw_B00634437_CW1#Party -->

    <owl:Class rdf:about="http://www.semanticweb.org/shawr/ontologies/2022/10/RyanShaw_B00634437_CW1#Party">
        <rdfs:subClassOf>
            <owl:Restriction>
                <owl:onProperty rdf:resource="http://www.semanticweb.org/shawr/ontologies/2022/10/RyanShaw_B00634437_CW1#hasAlignment"/>
                <owl:qualifiedCardinality rdf:datatype="http://www.w3.org/2001/XMLSchema#nonNegativeInteger">1</owl:qualifiedCardinality>
                <owl:onClass rdf:resource="http://www.semanticweb.org/shawr/ontologies/2022/10/RyanShaw_B00634437_CW1#PoliticalAlignment"/>
            </owl:Restriction>
        </rdfs:subClassOf>
        <rdfs:comment>The Party class represents the set of individual parties who had candidates standing in Belfast constituencies in the the 2019 general election.</rdfs:comment>
    </owl:Class>
    


    <!-- http://www.semanticweb.org/shawr/ontologies/2022/10/RyanShaw_B00634437_CW1#PeopleBeforeProfitCandidate -->

    <owl:Class rdf:about="http://www.semanticweb.org/shawr/ontologies/2022/10/RyanShaw_B00634437_CW1#PeopleBeforeProfitCandidate">
        <owl:equivalentClass>
            <owl:Class>
                <owl:intersectionOf rdf:parseType="Collection">
                    <rdf:Description rdf:about="http://www.semanticweb.org/shawr/ontologies/2022/10/RyanShaw_B00634437_CW1#Candidate"/>
                    <owl:Restriction>
                        <owl:onProperty rdf:resource="http://www.semanticweb.org/shawr/ontologies/2022/10/RyanShaw_B00634437_CW1#hasParty"/>
                        <owl:hasValue rdf:resource="http://www.semanticweb.org/shawr/ontologies/2022/10/RyanShaw_B00634437_CW1#PeopleBeforeProfit"/>
                    </owl:Restriction>
                </owl:intersectionOf>
            </owl:Class>
        </owl:equivalentClass>
        <rdfs:comment>The PeopleBeforeProfitCandidate class represents the set of individuals who are candidates for the PeopleBeforeProfit party in the 2019 general election.</rdfs:comment>
    </owl:Class>
    


    <!-- http://www.semanticweb.org/shawr/ontologies/2022/10/RyanShaw_B00634437_CW1#PoliticalAlignment -->

    <owl:Class rdf:about="http://www.semanticweb.org/shawr/ontologies/2022/10/RyanShaw_B00634437_CW1#PoliticalAlignment">
        <owl:equivalentClass>
            <owl:Class>
                <owl:oneOf rdf:parseType="Collection">
                    <rdf:Description rdf:about="http://www.semanticweb.org/shawr/ontologies/2022/10/RyanShaw_B00634437_CW1#Nationlist"/>
                    <rdf:Description rdf:about="http://www.semanticweb.org/shawr/ontologies/2022/10/RyanShaw_B00634437_CW1#Nondesignate"/>
                    <rdf:Description rdf:about="http://www.semanticweb.org/shawr/ontologies/2022/10/RyanShaw_B00634437_CW1#Unionist"/>
                </owl:oneOf>
            </owl:Class>
        </owl:equivalentClass>
        <rdfs:comment>The PoliticalAlignment class represents the different alignments of parties who stood in Belfast constituencies in the 2019 general election.</rdfs:comment>
    </owl:Class>
    


    <!-- http://www.semanticweb.org/shawr/ontologies/2022/10/RyanShaw_B00634437_CW1#SDLPCandidate -->

    <owl:Class rdf:about="http://www.semanticweb.org/shawr/ontologies/2022/10/RyanShaw_B00634437_CW1#SDLPCandidate">
        <owl:equivalentClass>
            <owl:Class>
                <owl:intersectionOf rdf:parseType="Collection">
                    <rdf:Description rdf:about="http://www.semanticweb.org/shawr/ontologies/2022/10/RyanShaw_B00634437_CW1#Candidate"/>
                    <owl:Restriction>
                        <owl:onProperty rdf:resource="http://www.semanticweb.org/shawr/ontologies/2022/10/RyanShaw_B00634437_CW1#hasParty"/>
                        <owl:hasValue rdf:resource="http://www.semanticweb.org/shawr/ontologies/2022/10/RyanShaw_B00634437_CW1#SDLP"/>
                    </owl:Restriction>
                </owl:intersectionOf>
            </owl:Class>
        </owl:equivalentClass>
        <rdfs:comment>The SDLPCandidate class represents the set of individuals who are candidates for the SDLP party in the 2019 general election.</rdfs:comment>
    </owl:Class>
    


    <!-- http://www.semanticweb.org/shawr/ontologies/2022/10/RyanShaw_B00634437_CW1#SDLPConstituency -->

    <owl:Class rdf:about="http://www.semanticweb.org/shawr/ontologies/2022/10/RyanShaw_B00634437_CW1#SDLPConstituency">
        <owl:equivalentClass>
            <owl:Class>
                <owl:intersectionOf rdf:parseType="Collection">
                    <rdf:Description rdf:about="http://www.semanticweb.org/shawr/ontologies/2022/10/RyanShaw_B00634437_CW1#Constituency"/>
                    <owl:Restriction>
                        <owl:onProperty rdf:resource="http://www.semanticweb.org/shawr/ontologies/2022/10/RyanShaw_B00634437_CW1#hasElectedParty"/>
                        <owl:hasValue rdf:resource="http://www.semanticweb.org/shawr/ontologies/2022/10/RyanShaw_B00634437_CW1#SDLP"/>
                    </owl:Restriction>
                </owl:intersectionOf>
            </owl:Class>
        </owl:equivalentClass>
        <rdfs:comment>The SDLPConstituency class represents the set of individual Belfast constituencies won by the SDLP party in the 2019 general election.</rdfs:comment>
    </owl:Class>
    


    <!-- http://www.semanticweb.org/shawr/ontologies/2022/10/RyanShaw_B00634437_CW1#SinnFeinCandidate -->

    <owl:Class rdf:about="http://www.semanticweb.org/shawr/ontologies/2022/10/RyanShaw_B00634437_CW1#SinnFeinCandidate">
        <owl:equivalentClass>
            <owl:Class>
                <owl:intersectionOf rdf:parseType="Collection">
                    <rdf:Description rdf:about="http://www.semanticweb.org/shawr/ontologies/2022/10/RyanShaw_B00634437_CW1#Candidate"/>
                    <owl:Restriction>
                        <owl:onProperty rdf:resource="http://www.semanticweb.org/shawr/ontologies/2022/10/RyanShaw_B00634437_CW1#hasParty"/>
                        <owl:hasValue rdf:resource="http://www.semanticweb.org/shawr/ontologies/2022/10/RyanShaw_B00634437_CW1#SinnFein"/>
                    </owl:Restriction>
                </owl:intersectionOf>
            </owl:Class>
        </owl:equivalentClass>
        <rdfs:comment>The SinnFeinCandidate class represents the set of individuals who are candidates for the SinnFein party in the 2019 general election.</rdfs:comment>
    </owl:Class>
    


    <!-- http://www.semanticweb.org/shawr/ontologies/2022/10/RyanShaw_B00634437_CW1#SinnFeinConstituency -->

    <owl:Class rdf:about="http://www.semanticweb.org/shawr/ontologies/2022/10/RyanShaw_B00634437_CW1#SinnFeinConstituency">
        <owl:equivalentClass>
            <owl:Class>
                <owl:intersectionOf rdf:parseType="Collection">
                    <rdf:Description rdf:about="http://www.semanticweb.org/shawr/ontologies/2022/10/RyanShaw_B00634437_CW1#Constituency"/>
                    <owl:Restriction>
                        <owl:onProperty rdf:resource="http://www.semanticweb.org/shawr/ontologies/2022/10/RyanShaw_B00634437_CW1#hasElectedParty"/>
                        <owl:hasValue rdf:resource="http://www.semanticweb.org/shawr/ontologies/2022/10/RyanShaw_B00634437_CW1#SinnFein"/>
                    </owl:Restriction>
                </owl:intersectionOf>
            </owl:Class>
        </owl:equivalentClass>
        <rdfs:comment>The SinnFeinConstituency class represents the set of individual Belfast constituencies won by the SinnFein party in the 2019 general election.</rdfs:comment>
    </owl:Class>
    


    <!-- http://www.semanticweb.org/shawr/ontologies/2022/10/RyanShaw_B00634437_CW1#UlsterUnionistCandidate -->

    <owl:Class rdf:about="http://www.semanticweb.org/shawr/ontologies/2022/10/RyanShaw_B00634437_CW1#UlsterUnionistCandidate">
        <owl:equivalentClass>
            <owl:Class>
                <owl:intersectionOf rdf:parseType="Collection">
                    <rdf:Description rdf:about="http://www.semanticweb.org/shawr/ontologies/2022/10/RyanShaw_B00634437_CW1#Candidate"/>
                    <owl:Restriction>
                        <owl:onProperty rdf:resource="http://www.semanticweb.org/shawr/ontologies/2022/10/RyanShaw_B00634437_CW1#hasParty"/>
                        <owl:hasValue rdf:resource="http://www.semanticweb.org/shawr/ontologies/2022/10/RyanShaw_B00634437_CW1#UlsterUnionist"/>
                    </owl:Restriction>
                </owl:intersectionOf>
            </owl:Class>
        </owl:equivalentClass>
        <rdfs:comment>The UlsterUnionistCandidate class represents the set of individuals who are candidates for the UlsterUnionist party in the 2019 general election.</rdfs:comment>
    </owl:Class>
    


    <!-- http://www.semanticweb.org/shawr/ontologies/2022/10/RyanShaw_B00634437_CW1#UnionistCandidate -->

    <owl:Class rdf:about="http://www.semanticweb.org/shawr/ontologies/2022/10/RyanShaw_B00634437_CW1#UnionistCandidate">
        <owl:equivalentClass>
            <owl:Class>
                <owl:intersectionOf rdf:parseType="Collection">
                    <rdf:Description rdf:about="http://www.semanticweb.org/shawr/ontologies/2022/10/RyanShaw_B00634437_CW1#Candidate"/>
                    <owl:Restriction>
                        <owl:onProperty rdf:resource="http://www.semanticweb.org/shawr/ontologies/2022/10/RyanShaw_B00634437_CW1#hasParty"/>
                        <owl:someValuesFrom rdf:resource="http://www.semanticweb.org/shawr/ontologies/2022/10/RyanShaw_B00634437_CW1#UnionistParty"/>
                    </owl:Restriction>
                </owl:intersectionOf>
            </owl:Class>
        </owl:equivalentClass>
        <rdfs:comment>The UnionistCandidate class represents the set of individuals who are candidates for parties with Unionist political alignment  in the 2019 general election.</rdfs:comment>
    </owl:Class>
    


    <!-- http://www.semanticweb.org/shawr/ontologies/2022/10/RyanShaw_B00634437_CW1#UnionistConstituency -->

    <owl:Class rdf:about="http://www.semanticweb.org/shawr/ontologies/2022/10/RyanShaw_B00634437_CW1#UnionistConstituency">
        <owl:equivalentClass>
            <owl:Class>
                <owl:intersectionOf rdf:parseType="Collection">
                    <rdf:Description rdf:about="http://www.semanticweb.org/shawr/ontologies/2022/10/RyanShaw_B00634437_CW1#Constituency"/>
                    <owl:Restriction>
                        <owl:onProperty rdf:resource="http://www.semanticweb.org/shawr/ontologies/2022/10/RyanShaw_B00634437_CW1#hasElectedParty"/>
                        <owl:someValuesFrom rdf:resource="http://www.semanticweb.org/shawr/ontologies/2022/10/RyanShaw_B00634437_CW1#UnionistParty"/>
                    </owl:Restriction>
                </owl:intersectionOf>
            </owl:Class>
        </owl:equivalentClass>
        <rdfs:comment>The UnionistConstituency class represents the set of individual Belfast constituencies won by parties with a Unionist political alignment in the 2019 general election.</rdfs:comment>
    </owl:Class>
    


    <!-- http://www.semanticweb.org/shawr/ontologies/2022/10/RyanShaw_B00634437_CW1#UnionistParty -->

    <owl:Class rdf:about="http://www.semanticweb.org/shawr/ontologies/2022/10/RyanShaw_B00634437_CW1#UnionistParty">
        <owl:equivalentClass>
            <owl:Class>
                <owl:intersectionOf rdf:parseType="Collection">
                    <rdf:Description rdf:about="http://www.semanticweb.org/shawr/ontologies/2022/10/RyanShaw_B00634437_CW1#Party"/>
                    <owl:Restriction>
                        <owl:onProperty rdf:resource="http://www.semanticweb.org/shawr/ontologies/2022/10/RyanShaw_B00634437_CW1#hasAlignment"/>
                        <owl:hasValue rdf:resource="http://www.semanticweb.org/shawr/ontologies/2022/10/RyanShaw_B00634437_CW1#Unionist"/>
                    </owl:Restriction>
                </owl:intersectionOf>
            </owl:Class>
        </owl:equivalentClass>
        <rdfs:comment>The UnionistParty class represents the set of individual parties who had a Unionist political alignment in the the 2019 general election.</rdfs:comment>
    </owl:Class>
    


    <!-- 
    ///////////////////////////////////////////////////////////////////////////////////////
    //
    // Individuals
    //
    ///////////////////////////////////////////////////////////////////////////////////////
     -->

    


    <!-- http://www.semanticweb.org/shawr/ontologies/2022/10/RyanShaw_B00634437_CW1#Alliance -->

    <owl:NamedIndividual rdf:about="http://www.semanticweb.org/shawr/ontologies/2022/10/RyanShaw_B00634437_CW1#Alliance">
        <rdf:type rdf:resource="http://www.semanticweb.org/shawr/ontologies/2022/10/RyanShaw_B00634437_CW1#Party"/>
        <hasAlignment rdf:resource="http://www.semanticweb.org/shawr/ontologies/2022/10/RyanShaw_B00634437_CW1#Nondesignate"/>
        <hasTotalAveragePercentageChangeOfVote rdf:datatype="http://www.w3.org/2001/XMLSchema#decimal">3.1</hasTotalAveragePercentageChangeOfVote>
        <hasTotalChangeInSeats rdf:datatype="http://www.w3.org/2001/XMLSchema#integer">0</hasTotalChangeInSeats>
        <hasTotalNumberOfCandidates rdf:datatype="http://www.w3.org/2001/XMLSchema#integer">4</hasTotalNumberOfCandidates>
        <hasTotalPercentageCandidateSuccessRate rdf:datatype="http://www.w3.org/2001/XMLSchema#integer">0</hasTotalPercentageCandidateSuccessRate>
        <hasTotalPercentageChangeInVote rdf:datatype="http://www.w3.org/2001/XMLSchema#decimal">12.5</hasTotalPercentageChangeInVote>
        <hasTotalPercentageShareOfVote rdf:datatype="http://www.w3.org/2001/XMLSchema#decimal">18.3</hasTotalPercentageShareOfVote>
        <hasTotalSeatsWon rdf:datatype="http://www.w3.org/2001/XMLSchema#integer">0</hasTotalSeatsWon>
        <hasTotalVoteCount rdf:datatype="http://www.w3.org/2001/XMLSchema#integer">32547</hasTotalVoteCount>
    </owl:NamedIndividual>
    


    <!-- http://www.semanticweb.org/shawr/ontologies/2022/10/RyanShaw_B00634437_CW1#Aontu -->

    <owl:NamedIndividual rdf:about="http://www.semanticweb.org/shawr/ontologies/2022/10/RyanShaw_B00634437_CW1#Aontu">
        <rdf:type rdf:resource="http://www.semanticweb.org/shawr/ontologies/2022/10/RyanShaw_B00634437_CW1#Party"/>
        <hasAlignment rdf:resource="http://www.semanticweb.org/shawr/ontologies/2022/10/RyanShaw_B00634437_CW1#Nationlist"/>
        <hasTotalAveragePercentageChangeOfVote rdf:datatype="http://www.w3.org/2001/XMLSchema#decimal">2.7</hasTotalAveragePercentageChangeOfVote>
        <hasTotalChangeInSeats rdf:datatype="http://www.w3.org/2001/XMLSchema#integer">0</hasTotalChangeInSeats>
        <hasTotalNumberOfCandidates rdf:datatype="http://www.w3.org/2001/XMLSchema#integer">2</hasTotalNumberOfCandidates>
        <hasTotalPercentageCandidateSuccessRate rdf:datatype="http://www.w3.org/2001/XMLSchema#integer">0</hasTotalPercentageCandidateSuccessRate>
        <hasTotalPercentageChangeInVote rdf:datatype="http://www.w3.org/2001/XMLSchema#decimal">5.4</hasTotalPercentageChangeInVote>
        <hasTotalPercentageShareOfVote rdf:datatype="http://www.w3.org/2001/XMLSchema#decimal">1.2</hasTotalPercentageShareOfVote>
        <hasTotalSeatsWon rdf:datatype="http://www.w3.org/2001/XMLSchema#integer">0</hasTotalSeatsWon>
        <hasTotalVoteCount rdf:datatype="http://www.w3.org/2001/XMLSchema#integer">2185</hasTotalVoteCount>
    </owl:NamedIndividual>
    


    <!-- http://www.semanticweb.org/shawr/ontologies/2022/10/RyanShaw_B00634437_CW1#BelfastEast -->

    <owl:NamedIndividual rdf:about="http://www.semanticweb.org/shawr/ontologies/2022/10/RyanShaw_B00634437_CW1#BelfastEast">
        <rdf:type rdf:resource="http://www.semanticweb.org/shawr/ontologies/2022/10/RyanShaw_B00634437_CW1#Constituency"/>
        <hasElectedParty rdf:resource="http://www.semanticweb.org/shawr/ontologies/2022/10/RyanShaw_B00634437_CW1#DUP"/>
        <hasElectorate rdf:datatype="http://www.w3.org/2001/XMLSchema#integer">66245</hasElectorate>
        <hasMajority rdf:datatype="http://www.w3.org/2001/XMLSchema#integer">1819</hasMajority>
        <hasOutcomeStatus>Hold</hasOutcomeStatus>
        <hasTurnout rdf:datatype="http://www.w3.org/2001/XMLSchema#decimal">64.1</hasTurnout>
    </owl:NamedIndividual>
    


    <!-- http://www.semanticweb.org/shawr/ontologies/2022/10/RyanShaw_B00634437_CW1#BelfastNorth -->

    <owl:NamedIndividual rdf:about="http://www.semanticweb.org/shawr/ontologies/2022/10/RyanShaw_B00634437_CW1#BelfastNorth">
        <rdf:type rdf:resource="http://www.semanticweb.org/shawr/ontologies/2022/10/RyanShaw_B00634437_CW1#Constituency"/>
        <hasElectedParty rdf:resource="http://www.semanticweb.org/shawr/ontologies/2022/10/RyanShaw_B00634437_CW1#SinnFein"/>
        <hasElectorate rdf:datatype="http://www.w3.org/2001/XMLSchema#integer">72225</hasElectorate>
        <hasMajority rdf:datatype="http://www.w3.org/2001/XMLSchema#integer">1943</hasMajority>
        <hasOutcomeStatus>Gain</hasOutcomeStatus>
        <hasTurnout rdf:datatype="http://www.w3.org/2001/XMLSchema#decimal">67.9</hasTurnout>
    </owl:NamedIndividual>
    


    <!-- http://www.semanticweb.org/shawr/ontologies/2022/10/RyanShaw_B00634437_CW1#BelfastSouth -->

    <owl:NamedIndividual rdf:about="http://www.semanticweb.org/shawr/ontologies/2022/10/RyanShaw_B00634437_CW1#BelfastSouth">
        <rdf:type rdf:resource="http://www.semanticweb.org/shawr/ontologies/2022/10/RyanShaw_B00634437_CW1#Constituency"/>
        <hasElectedParty rdf:resource="http://www.semanticweb.org/shawr/ontologies/2022/10/RyanShaw_B00634437_CW1#SDLP"/>
        <hasElectorate rdf:datatype="http://www.w3.org/2001/XMLSchema#integer">69984</hasElectorate>
        <hasMajority rdf:datatype="http://www.w3.org/2001/XMLSchema#integer">15401</hasMajority>
        <hasOutcomeStatus>Gain</hasOutcomeStatus>
        <hasTurnout rdf:datatype="http://www.w3.org/2001/XMLSchema#decimal">67.7</hasTurnout>
    </owl:NamedIndividual>
    


    <!-- http://www.semanticweb.org/shawr/ontologies/2022/10/RyanShaw_B00634437_CW1#BelfastWest -->

    <owl:NamedIndividual rdf:about="http://www.semanticweb.org/shawr/ontologies/2022/10/RyanShaw_B00634437_CW1#BelfastWest">
        <rdf:type rdf:resource="http://www.semanticweb.org/shawr/ontologies/2022/10/RyanShaw_B00634437_CW1#Constituency"/>
        <hasElectedParty rdf:resource="http://www.semanticweb.org/shawr/ontologies/2022/10/RyanShaw_B00634437_CW1#SinnFein"/>
        <hasElectorate rdf:datatype="http://www.w3.org/2001/XMLSchema#integer">65644</hasElectorate>
        <hasMajority rdf:datatype="http://www.w3.org/2001/XMLSchema#integer">14672</hasMajority>
        <hasOutcomeStatus>Hold</hasOutcomeStatus>
        <hasTurnout rdf:datatype="http://www.w3.org/2001/XMLSchema#decimal">59.1</hasTurnout>
    </owl:NamedIndividual>
    


    <!-- http://www.semanticweb.org/shawr/ontologies/2022/10/RyanShaw_B00634437_CW1#CarlMcClean -->

    <owl:NamedIndividual rdf:about="http://www.semanticweb.org/shawr/ontologies/2022/10/RyanShaw_B00634437_CW1#CarlMcClean">
        <rdf:type rdf:resource="http://www.semanticweb.org/shawr/ontologies/2022/10/RyanShaw_B00634437_CW1#Candidate"/>
        <hasConstituency rdf:resource="http://www.semanticweb.org/shawr/ontologies/2022/10/RyanShaw_B00634437_CW1#BelfastEast"/>
        <hasParty rdf:resource="http://www.semanticweb.org/shawr/ontologies/2022/10/RyanShaw_B00634437_CW1#UlsterUnionist"/>
        <hasPercentageChangeInVote rdf:datatype="http://www.w3.org/2001/XMLSchema#decimal">2.6</hasPercentageChangeInVote>
        <hasPercentageShareOfVote rdf:datatype="http://www.w3.org/2001/XMLSchema#decimal">5.9</hasPercentageShareOfVote>
        <hasVoteCount rdf:datatype="http://www.w3.org/2001/XMLSchema#integer">2516</hasVoteCount>
    </owl:NamedIndividual>
    


    <!-- http://www.semanticweb.org/shawr/ontologies/2022/10/RyanShaw_B00634437_CW1#ChrisMcHugh -->

    <owl:NamedIndividual rdf:about="http://www.semanticweb.org/shawr/ontologies/2022/10/RyanShaw_B00634437_CW1#ChrisMcHugh">
        <rdf:type rdf:resource="http://www.semanticweb.org/shawr/ontologies/2022/10/RyanShaw_B00634437_CW1#Candidate"/>
        <hasConstituency rdf:resource="http://www.semanticweb.org/shawr/ontologies/2022/10/RyanShaw_B00634437_CW1#BelfastSouth"/>
        <hasParty rdf:resource="http://www.semanticweb.org/shawr/ontologies/2022/10/RyanShaw_B00634437_CW1#Aontu"/>
        <hasPercentageChangeInVote rdf:datatype="http://www.w3.org/2001/XMLSchema#decimal">1.2</hasPercentageChangeInVote>
        <hasPercentageShareOfVote rdf:datatype="http://www.w3.org/2001/XMLSchema#decimal">1.2</hasPercentageShareOfVote>
        <hasVoteCount rdf:datatype="http://www.w3.org/2001/XMLSchema#integer">550</hasVoteCount>
    </owl:NamedIndividual>
    


    <!-- http://www.semanticweb.org/shawr/ontologies/2022/10/RyanShaw_B00634437_CW1#ClaireHanna -->

    <owl:NamedIndividual rdf:about="http://www.semanticweb.org/shawr/ontologies/2022/10/RyanShaw_B00634437_CW1#ClaireHanna">
        <rdf:type rdf:resource="http://www.semanticweb.org/shawr/ontologies/2022/10/RyanShaw_B00634437_CW1#Candidate"/>
        <hasConstituency rdf:resource="http://www.semanticweb.org/shawr/ontologies/2022/10/RyanShaw_B00634437_CW1#BelfastSouth"/>
        <hasMoreVotesThan rdf:resource="http://www.semanticweb.org/shawr/ontologies/2022/10/RyanShaw_B00634437_CW1#ChrisMcHugh"/>
        <hasMoreVotesThan rdf:resource="http://www.semanticweb.org/shawr/ontologies/2022/10/RyanShaw_B00634437_CW1#EmmaLittlePengelly"/>
        <hasMoreVotesThan rdf:resource="http://www.semanticweb.org/shawr/ontologies/2022/10/RyanShaw_B00634437_CW1#MichaelHenderson"/>
        <hasMoreVotesThan rdf:resource="http://www.semanticweb.org/shawr/ontologies/2022/10/RyanShaw_B00634437_CW1#PaulaBradshaw"/>
        <hasParty rdf:resource="http://www.semanticweb.org/shawr/ontologies/2022/10/RyanShaw_B00634437_CW1#SDLP"/>
        <hasPercentageChangeInVote rdf:datatype="http://www.w3.org/2001/XMLSchema#decimal">31.3</hasPercentageChangeInVote>
        <hasPercentageShareOfVote rdf:datatype="http://www.w3.org/2001/XMLSchema#decimal">57.2</hasPercentageShareOfVote>
        <hasVoteCount rdf:datatype="http://www.w3.org/2001/XMLSchema#integer">27079</hasVoteCount>
    </owl:NamedIndividual>
    


    <!-- http://www.semanticweb.org/shawr/ontologies/2022/10/RyanShaw_B00634437_CW1#DUP -->

    <owl:NamedIndividual rdf:about="http://www.semanticweb.org/shawr/ontologies/2022/10/RyanShaw_B00634437_CW1#DUP">
        <rdf:type rdf:resource="http://www.semanticweb.org/shawr/ontologies/2022/10/RyanShaw_B00634437_CW1#Party"/>
        <hasAlignment rdf:resource="http://www.semanticweb.org/shawr/ontologies/2022/10/RyanShaw_B00634437_CW1#Unionist"/>
        <hasTotalAveragePercentageChangeOfVote rdf:datatype="http://www.w3.org/2001/XMLSchema#decimal">-3.9</hasTotalAveragePercentageChangeOfVote>
        <hasTotalChangeInSeats rdf:datatype="http://www.w3.org/2001/XMLSchema#integer">-2</hasTotalChangeInSeats>
        <hasTotalNumberOfCandidates rdf:datatype="http://www.w3.org/2001/XMLSchema#integer">4</hasTotalNumberOfCandidates>
        <hasTotalPercentageCandidateSuccessRate rdf:datatype="http://www.w3.org/2001/XMLSchema#integer">25</hasTotalPercentageCandidateSuccessRate>
        <hasTotalPercentageChangeInVote rdf:datatype="http://www.w3.org/2001/XMLSchema#decimal">-15.5</hasTotalPercentageChangeInVote>
        <hasTotalPercentageShareOfVote rdf:datatype="http://www.w3.org/2001/XMLSchema#decimal">33.2</hasTotalPercentageShareOfVote>
        <hasTotalSeatsWon rdf:datatype="http://www.w3.org/2001/XMLSchema#integer">1</hasTotalSeatsWon>
        <hasTotalVoteCount rdf:datatype="http://www.w3.org/2001/XMLSchema#integer">58907</hasTotalVoteCount>
    </owl:NamedIndividual>
    


    <!-- http://www.semanticweb.org/shawr/ontologies/2022/10/RyanShaw_B00634437_CW1#DonnamarieHiggins -->

    <owl:NamedIndividual rdf:about="http://www.semanticweb.org/shawr/ontologies/2022/10/RyanShaw_B00634437_CW1#DonnamarieHiggins">
        <rdf:type rdf:resource="http://www.semanticweb.org/shawr/ontologies/2022/10/RyanShaw_B00634437_CW1#Candidate"/>
        <hasConstituency rdf:resource="http://www.semanticweb.org/shawr/ontologies/2022/10/RyanShaw_B00634437_CW1#BelfastWest"/>
        <hasParty rdf:resource="http://www.semanticweb.org/shawr/ontologies/2022/10/RyanShaw_B00634437_CW1#Alliance"/>
        <hasPercentageChangeInVote rdf:datatype="http://www.w3.org/2001/XMLSchema#decimal">3.1</hasPercentageChangeInVote>
        <hasPercentageShareOfVote rdf:datatype="http://www.w3.org/2001/XMLSchema#integer">1882</hasPercentageShareOfVote>
        <hasPercentageShareOfVote rdf:datatype="http://www.w3.org/2001/XMLSchema#decimal">4.9</hasPercentageShareOfVote>
    </owl:NamedIndividual>
    


    <!-- http://www.semanticweb.org/shawr/ontologies/2022/10/RyanShaw_B00634437_CW1#EmmaLittlePengelly -->

    <owl:NamedIndividual rdf:about="http://www.semanticweb.org/shawr/ontologies/2022/10/RyanShaw_B00634437_CW1#EmmaLittlePengelly">
        <rdf:type rdf:resource="http://www.semanticweb.org/shawr/ontologies/2022/10/RyanShaw_B00634437_CW1#Candidate"/>
        <hasConstituency rdf:resource="http://www.semanticweb.org/shawr/ontologies/2022/10/RyanShaw_B00634437_CW1#BelfastSouth"/>
        <hasParty rdf:resource="http://www.semanticweb.org/shawr/ontologies/2022/10/RyanShaw_B00634437_CW1#DUP"/>
        <hasPercentageChangeInVote rdf:datatype="http://www.w3.org/2001/XMLSchema#decimal">-5.8</hasPercentageChangeInVote>
        <hasPercentageShareOfVote rdf:datatype="http://www.w3.org/2001/XMLSchema#decimal">24.7</hasPercentageShareOfVote>
        <hasVoteCount rdf:datatype="http://www.w3.org/2001/XMLSchema#integer">11678</hasVoteCount>
    </owl:NamedIndividual>
    


    <!-- http://www.semanticweb.org/shawr/ontologies/2022/10/RyanShaw_B00634437_CW1#FrankMcCoubrey -->

    <owl:NamedIndividual rdf:about="http://www.semanticweb.org/shawr/ontologies/2022/10/RyanShaw_B00634437_CW1#FrankMcCoubrey">
        <rdf:type rdf:resource="http://www.semanticweb.org/shawr/ontologies/2022/10/RyanShaw_B00634437_CW1#Candidate"/>
        <hasConstituency rdf:resource="http://www.semanticweb.org/shawr/ontologies/2022/10/RyanShaw_B00634437_CW1#BelfastWest"/>
        <hasParty rdf:resource="http://www.semanticweb.org/shawr/ontologies/2022/10/RyanShaw_B00634437_CW1#DUP"/>
        <hasPercentageChangeInVote rdf:datatype="http://www.w3.org/2001/XMLSchema#decimal">0.0</hasPercentageChangeInVote>
        <hasPercentageShareOfVote rdf:datatype="http://www.w3.org/2001/XMLSchema#decimal">13.5</hasPercentageShareOfVote>
        <hasVoteCount rdf:datatype="http://www.w3.org/2001/XMLSchema#integer">5220</hasVoteCount>
    </owl:NamedIndividual>
    


    <!-- http://www.semanticweb.org/shawr/ontologies/2022/10/RyanShaw_B00634437_CW1#GavinRobinson -->

    <owl:NamedIndividual rdf:about="http://www.semanticweb.org/shawr/ontologies/2022/10/RyanShaw_B00634437_CW1#GavinRobinson">
        <rdf:type rdf:resource="http://www.semanticweb.org/shawr/ontologies/2022/10/RyanShaw_B00634437_CW1#Candidate"/>
        <hasConstituency rdf:resource="http://www.semanticweb.org/shawr/ontologies/2022/10/RyanShaw_B00634437_CW1#BelfastEast"/>
        <hasMoreVotesThan rdf:resource="http://www.semanticweb.org/shawr/ontologies/2022/10/RyanShaw_B00634437_CW1#CarlMcClean"/>
        <hasMoreVotesThan rdf:resource="http://www.semanticweb.org/shawr/ontologies/2022/10/RyanShaw_B00634437_CW1#NaomiLong"/>
        <hasParty rdf:resource="http://www.semanticweb.org/shawr/ontologies/2022/10/RyanShaw_B00634437_CW1#DUP"/>
        <hasPercentageChangeInVote rdf:datatype="http://www.w3.org/2001/XMLSchema#decimal">-6.6</hasPercentageChangeInVote>
        <hasPercentageShareOfVote rdf:datatype="http://www.w3.org/2001/XMLSchema#decimal">49.2</hasPercentageShareOfVote>
        <hasVoteCount rdf:datatype="http://www.w3.org/2001/XMLSchema#integer">20874</hasVoteCount>
    </owl:NamedIndividual>
    


    <!-- http://www.semanticweb.org/shawr/ontologies/2022/10/RyanShaw_B00634437_CW1#GerryCarroll -->

    <owl:NamedIndividual rdf:about="http://www.semanticweb.org/shawr/ontologies/2022/10/RyanShaw_B00634437_CW1#GerryCarroll">
        <rdf:type rdf:resource="http://www.semanticweb.org/shawr/ontologies/2022/10/RyanShaw_B00634437_CW1#Candidate"/>
        <hasConstituency rdf:resource="http://www.semanticweb.org/shawr/ontologies/2022/10/RyanShaw_B00634437_CW1#BelfastWest"/>
        <hasParty rdf:resource="http://www.semanticweb.org/shawr/ontologies/2022/10/RyanShaw_B00634437_CW1#PeopleBeforeProfit"/>
        <hasPercentageChangeInVote rdf:datatype="http://www.w3.org/2001/XMLSchema#decimal">5.8</hasPercentageChangeInVote>
        <hasPercentageShareOfVote rdf:datatype="http://www.w3.org/2001/XMLSchema#decimal">16.0</hasPercentageShareOfVote>
        <hasVoteCount rdf:datatype="http://www.w3.org/2001/XMLSchema#integer">6194</hasVoteCount>
    </owl:NamedIndividual>
    


    <!-- http://www.semanticweb.org/shawr/ontologies/2022/10/RyanShaw_B00634437_CW1#JohnFinucane -->

    <owl:NamedIndividual rdf:about="http://www.semanticweb.org/shawr/ontologies/2022/10/RyanShaw_B00634437_CW1#JohnFinucane">
        <rdf:type rdf:resource="http://www.semanticweb.org/shawr/ontologies/2022/10/RyanShaw_B00634437_CW1#Candidate"/>
        <hasConstituency rdf:resource="http://www.semanticweb.org/shawr/ontologies/2022/10/RyanShaw_B00634437_CW1#BelfastNorth"/>
        <hasMoreVotesThan rdf:resource="http://www.semanticweb.org/shawr/ontologies/2022/10/RyanShaw_B00634437_CW1#NigelDodds"/>
        <hasMoreVotesThan rdf:resource="http://www.semanticweb.org/shawr/ontologies/2022/10/RyanShaw_B00634437_CW1#NualaMcAllister"/>
        <hasParty rdf:resource="http://www.semanticweb.org/shawr/ontologies/2022/10/RyanShaw_B00634437_CW1#SinnFein"/>
        <hasPercentageChangeInVote rdf:datatype="http://www.w3.org/2001/XMLSchema#decimal">5.4</hasPercentageChangeInVote>
        <hasPercentageShareOfVote rdf:datatype="http://www.w3.org/2001/XMLSchema#decimal">47.1</hasPercentageShareOfVote>
        <hasVoteCount rdf:datatype="http://www.w3.org/2001/XMLSchema#integer">23078</hasVoteCount>
    </owl:NamedIndividual>
    


    <!-- http://www.semanticweb.org/shawr/ontologies/2022/10/RyanShaw_B00634437_CW1#MichaelHenderson -->

    <owl:NamedIndividual rdf:about="http://www.semanticweb.org/shawr/ontologies/2022/10/RyanShaw_B00634437_CW1#MichaelHenderson">
        <rdf:type rdf:resource="http://www.semanticweb.org/shawr/ontologies/2022/10/RyanShaw_B00634437_CW1#Candidate"/>
        <hasConstituency rdf:resource="http://www.semanticweb.org/shawr/ontologies/2022/10/RyanShaw_B00634437_CW1#BelfastSouth"/>
        <hasParty rdf:resource="http://www.semanticweb.org/shawr/ontologies/2022/10/RyanShaw_B00634437_CW1#UlsterUnionist"/>
        <hasPercentageChangeInVote rdf:datatype="http://www.w3.org/2001/XMLSchema#decimal">-0.8</hasPercentageChangeInVote>
        <hasPercentageShareOfVote rdf:datatype="http://www.w3.org/2001/XMLSchema#decimal">2.7</hasPercentageShareOfVote>
        <hasVoteCount rdf:datatype="http://www.w3.org/2001/XMLSchema#integer">1259</hasVoteCount>
    </owl:NamedIndividual>
    


    <!-- http://www.semanticweb.org/shawr/ontologies/2022/10/RyanShaw_B00634437_CW1#MonicaDigney -->

    <owl:NamedIndividual rdf:about="http://www.semanticweb.org/shawr/ontologies/2022/10/RyanShaw_B00634437_CW1#MonicaDigney">
        <rdf:type rdf:resource="http://www.semanticweb.org/shawr/ontologies/2022/10/RyanShaw_B00634437_CW1#Candidate"/>
        <hasConstituency rdf:resource="http://www.semanticweb.org/shawr/ontologies/2022/10/RyanShaw_B00634437_CW1#BelfastWest"/>
        <hasParty rdf:resource="http://www.semanticweb.org/shawr/ontologies/2022/10/RyanShaw_B00634437_CW1#Aontu"/>
        <hasPercentageChangeInVote rdf:datatype="http://www.w3.org/2001/XMLSchema#decimal">4.2</hasPercentageChangeInVote>
        <hasPercentageShareOfVote rdf:datatype="http://www.w3.org/2001/XMLSchema#decimal">4.2</hasPercentageShareOfVote>
        <hasVoteCount rdf:datatype="http://www.w3.org/2001/XMLSchema#integer">1635</hasVoteCount>
    </owl:NamedIndividual>
    


    <!-- http://www.semanticweb.org/shawr/ontologies/2022/10/RyanShaw_B00634437_CW1#NaomiLong -->

    <owl:NamedIndividual rdf:about="http://www.semanticweb.org/shawr/ontologies/2022/10/RyanShaw_B00634437_CW1#NaomiLong">
        <rdf:type rdf:resource="http://www.semanticweb.org/shawr/ontologies/2022/10/RyanShaw_B00634437_CW1#Candidate"/>
        <hasConstituency rdf:resource="http://www.semanticweb.org/shawr/ontologies/2022/10/RyanShaw_B00634437_CW1#BelfastEast"/>
        <hasParty rdf:resource="http://www.semanticweb.org/shawr/ontologies/2022/10/RyanShaw_B00634437_CW1#Alliance"/>
        <hasPercentageChangeInVote rdf:datatype="http://www.w3.org/2001/XMLSchema#decimal">8.9</hasPercentageChangeInVote>
        <hasPercentageShareOfVote rdf:datatype="http://www.w3.org/2001/XMLSchema#decimal">44.9</hasPercentageShareOfVote>
        <hasVoteCount rdf:datatype="http://www.w3.org/2001/XMLSchema#integer">19055</hasVoteCount>
    </owl:NamedIndividual>
    


    <!-- http://www.semanticweb.org/shawr/ontologies/2022/10/RyanShaw_B00634437_CW1#Nationlist -->

    <owl:NamedIndividual rdf:about="http://www.semanticweb.org/shawr/ontologies/2022/10/RyanShaw_B00634437_CW1#Nationlist"/>
    


    <!-- http://www.semanticweb.org/shawr/ontologies/2022/10/RyanShaw_B00634437_CW1#NigelDodds -->

    <owl:NamedIndividual rdf:about="http://www.semanticweb.org/shawr/ontologies/2022/10/RyanShaw_B00634437_CW1#NigelDodds">
        <rdf:type rdf:resource="http://www.semanticweb.org/shawr/ontologies/2022/10/RyanShaw_B00634437_CW1#Candidate"/>
        <hasConstituency rdf:resource="http://www.semanticweb.org/shawr/ontologies/2022/10/RyanShaw_B00634437_CW1#BelfastNorth"/>
        <hasParty rdf:resource="http://www.semanticweb.org/shawr/ontologies/2022/10/RyanShaw_B00634437_CW1#DUP"/>
        <hasPercentageChangeInVote rdf:datatype="http://www.w3.org/2001/XMLSchema#decimal">-3.1</hasPercentageChangeInVote>
        <hasPercentageShareOfVote rdf:datatype="http://www.w3.org/2001/XMLSchema#decimal">43.1</hasPercentageShareOfVote>
        <hasVoteCount rdf:datatype="http://www.w3.org/2001/XMLSchema#integer">21135</hasVoteCount>
    </owl:NamedIndividual>
    


    <!-- http://www.semanticweb.org/shawr/ontologies/2022/10/RyanShaw_B00634437_CW1#Nondesignate -->

    <owl:NamedIndividual rdf:about="http://www.semanticweb.org/shawr/ontologies/2022/10/RyanShaw_B00634437_CW1#Nondesignate"/>
    


    <!-- http://www.semanticweb.org/shawr/ontologies/2022/10/RyanShaw_B00634437_CW1#NualaMcAllister -->

    <owl:NamedIndividual rdf:about="http://www.semanticweb.org/shawr/ontologies/2022/10/RyanShaw_B00634437_CW1#NualaMcAllister">
        <rdf:type rdf:resource="http://www.semanticweb.org/shawr/ontologies/2022/10/RyanShaw_B00634437_CW1#Candidate"/>
        <hasConstituency rdf:resource="http://www.semanticweb.org/shawr/ontologies/2022/10/RyanShaw_B00634437_CW1#BelfastNorth"/>
        <hasParty rdf:resource="http://www.semanticweb.org/shawr/ontologies/2022/10/RyanShaw_B00634437_CW1#Alliance"/>
        <hasPercentageChangeInVote rdf:datatype="http://www.w3.org/2001/XMLSchema#decimal">4.4</hasPercentageChangeInVote>
        <hasPercentageShareOfVote rdf:datatype="http://www.w3.org/2001/XMLSchema#decimal">9.8</hasPercentageShareOfVote>
        <hasVoteCount rdf:datatype="http://www.w3.org/2001/XMLSchema#integer">4824</hasVoteCount>
    </owl:NamedIndividual>
    


    <!-- http://www.semanticweb.org/shawr/ontologies/2022/10/RyanShaw_B00634437_CW1#PaulDoherty -->

    <owl:NamedIndividual rdf:about="http://www.semanticweb.org/shawr/ontologies/2022/10/RyanShaw_B00634437_CW1#PaulDoherty">
        <rdf:type rdf:resource="http://www.semanticweb.org/shawr/ontologies/2022/10/RyanShaw_B00634437_CW1#Candidate"/>
        <hasConstituency rdf:resource="http://www.semanticweb.org/shawr/ontologies/2022/10/RyanShaw_B00634437_CW1#BelfastWest"/>
        <hasParty rdf:resource="http://www.semanticweb.org/shawr/ontologies/2022/10/RyanShaw_B00634437_CW1#SDLP"/>
        <hasPercentageChangeInVote rdf:datatype="http://www.w3.org/2001/XMLSchema#decimal">0.7</hasPercentageChangeInVote>
        <hasPercentageShareOfVote rdf:datatype="http://www.w3.org/2001/XMLSchema#decimal">7.7</hasPercentageShareOfVote>
        <hasVoteCount rdf:datatype="http://www.w3.org/2001/XMLSchema#integer">2985</hasVoteCount>
    </owl:NamedIndividual>
    


    <!-- http://www.semanticweb.org/shawr/ontologies/2022/10/RyanShaw_B00634437_CW1#PaulMaskey -->

    <owl:NamedIndividual rdf:about="http://www.semanticweb.org/shawr/ontologies/2022/10/RyanShaw_B00634437_CW1#PaulMaskey">
        <rdf:type rdf:resource="http://www.semanticweb.org/shawr/ontologies/2022/10/RyanShaw_B00634437_CW1#Candidate"/>
        <hasConstituency rdf:resource="http://www.semanticweb.org/shawr/ontologies/2022/10/RyanShaw_B00634437_CW1#BelfastWest"/>
        <hasMoreVotesThan rdf:resource="http://www.semanticweb.org/shawr/ontologies/2022/10/RyanShaw_B00634437_CW1#DonnamarieHiggins"/>
        <hasMoreVotesThan rdf:resource="http://www.semanticweb.org/shawr/ontologies/2022/10/RyanShaw_B00634437_CW1#FrankMcCoubrey"/>
        <hasMoreVotesThan rdf:resource="http://www.semanticweb.org/shawr/ontologies/2022/10/RyanShaw_B00634437_CW1#GerryCarroll"/>
        <hasMoreVotesThan rdf:resource="http://www.semanticweb.org/shawr/ontologies/2022/10/RyanShaw_B00634437_CW1#MonicaDigney"/>
        <hasMoreVotesThan rdf:resource="http://www.semanticweb.org/shawr/ontologies/2022/10/RyanShaw_B00634437_CW1#PaulDoherty"/>
        <hasParty rdf:resource="http://www.semanticweb.org/shawr/ontologies/2022/10/RyanShaw_B00634437_CW1#SinnFein"/>
        <hasPercentageChangeInVote rdf:datatype="http://www.w3.org/2001/XMLSchema#decimal">-12.9</hasPercentageChangeInVote>
        <hasPercentageShareOfVote rdf:datatype="http://www.w3.org/2001/XMLSchema#decimal">53.8</hasPercentageShareOfVote>
        <hasVoteCount rdf:datatype="http://www.w3.org/2001/XMLSchema#integer">20866</hasVoteCount>
    </owl:NamedIndividual>
    


    <!-- http://www.semanticweb.org/shawr/ontologies/2022/10/RyanShaw_B00634437_CW1#PaulaBradshaw -->

    <owl:NamedIndividual rdf:about="http://www.semanticweb.org/shawr/ontologies/2022/10/RyanShaw_B00634437_CW1#PaulaBradshaw">
        <rdf:type rdf:resource="http://www.semanticweb.org/shawr/ontologies/2022/10/RyanShaw_B00634437_CW1#Candidate"/>
        <hasConstituency rdf:resource="http://www.semanticweb.org/shawr/ontologies/2022/10/RyanShaw_B00634437_CW1#BelfastSouth"/>
        <hasParty rdf:resource="http://www.semanticweb.org/shawr/ontologies/2022/10/RyanShaw_B00634437_CW1#Alliance"/>
        <hasPercentageChangeInVote rdf:datatype="http://www.w3.org/2001/XMLSchema#decimal">-3.9</hasPercentageChangeInVote>
        <hasPercentageShareOfVote rdf:datatype="http://www.w3.org/2001/XMLSchema#decimal">14.3</hasPercentageShareOfVote>
        <hasVoteCount rdf:datatype="http://www.w3.org/2001/XMLSchema#integer">6786</hasVoteCount>
    </owl:NamedIndividual>
    


    <!-- http://www.semanticweb.org/shawr/ontologies/2022/10/RyanShaw_B00634437_CW1#PeopleBeforeProfit -->

    <owl:NamedIndividual rdf:about="http://www.semanticweb.org/shawr/ontologies/2022/10/RyanShaw_B00634437_CW1#PeopleBeforeProfit">
        <rdf:type rdf:resource="http://www.semanticweb.org/shawr/ontologies/2022/10/RyanShaw_B00634437_CW1#Party"/>
        <hasAlignment rdf:resource="http://www.semanticweb.org/shawr/ontologies/2022/10/RyanShaw_B00634437_CW1#Nationlist"/>
        <hasTotalAveragePercentageChangeOfVote rdf:datatype="http://www.w3.org/2001/XMLSchema#decimal">5.8</hasTotalAveragePercentageChangeOfVote>
        <hasTotalChangeInSeats rdf:datatype="http://www.w3.org/2001/XMLSchema#integer">0</hasTotalChangeInSeats>
        <hasTotalNumberOfCandidates rdf:datatype="http://www.w3.org/2001/XMLSchema#integer">1</hasTotalNumberOfCandidates>
        <hasTotalPercentageCandidateSuccessRate rdf:datatype="http://www.w3.org/2001/XMLSchema#integer">0</hasTotalPercentageCandidateSuccessRate>
        <hasTotalPercentageChangeInVote rdf:datatype="http://www.w3.org/2001/XMLSchema#decimal">5.8</hasTotalPercentageChangeInVote>
        <hasTotalPercentageShareOfVote rdf:datatype="http://www.w3.org/2001/XMLSchema#decimal">3.5</hasTotalPercentageShareOfVote>
        <hasTotalSeatsWon rdf:datatype="http://www.w3.org/2001/XMLSchema#integer">0</hasTotalSeatsWon>
        <hasTotalVoteCount rdf:datatype="http://www.w3.org/2001/XMLSchema#integer">6194</hasTotalVoteCount>
    </owl:NamedIndividual>
    


    <!-- http://www.semanticweb.org/shawr/ontologies/2022/10/RyanShaw_B00634437_CW1#SDLP -->

    <owl:NamedIndividual rdf:about="http://www.semanticweb.org/shawr/ontologies/2022/10/RyanShaw_B00634437_CW1#SDLP">
        <rdf:type rdf:resource="http://www.semanticweb.org/shawr/ontologies/2022/10/RyanShaw_B00634437_CW1#Party"/>
        <hasAlignment rdf:resource="http://www.semanticweb.org/shawr/ontologies/2022/10/RyanShaw_B00634437_CW1#Nationlist"/>
        <hasTotalAveragePercentageChangeOfVote rdf:datatype="http://www.w3.org/2001/XMLSchema#decimal">16.0</hasTotalAveragePercentageChangeOfVote>
        <hasTotalChangeInSeats rdf:datatype="http://www.w3.org/2001/XMLSchema#integer">1</hasTotalChangeInSeats>
        <hasTotalNumberOfCandidates rdf:datatype="http://www.w3.org/2001/XMLSchema#integer">2</hasTotalNumberOfCandidates>
        <hasTotalPercentageCandidateSuccessRate rdf:datatype="http://www.w3.org/2001/XMLSchema#integer">50</hasTotalPercentageCandidateSuccessRate>
        <hasTotalPercentageChangeInVote rdf:datatype="http://www.w3.org/2001/XMLSchema#decimal">32.0</hasTotalPercentageChangeInVote>
        <hasTotalPercentageShareOfVote rdf:datatype="http://www.w3.org/2001/XMLSchema#decimal">16.9</hasTotalPercentageShareOfVote>
        <hasTotalSeatsWon rdf:datatype="http://www.w3.org/2001/XMLSchema#integer">1</hasTotalSeatsWon>
        <hasTotalVoteCount rdf:datatype="http://www.w3.org/2001/XMLSchema#integer">30064</hasTotalVoteCount>
    </owl:NamedIndividual>
    


    <!-- http://www.semanticweb.org/shawr/ontologies/2022/10/RyanShaw_B00634437_CW1#SinnFein -->

    <owl:NamedIndividual rdf:about="http://www.semanticweb.org/shawr/ontologies/2022/10/RyanShaw_B00634437_CW1#SinnFein">
        <rdf:type rdf:resource="http://www.semanticweb.org/shawr/ontologies/2022/10/RyanShaw_B00634437_CW1#Party"/>
        <hasAlignment rdf:resource="http://www.semanticweb.org/shawr/ontologies/2022/10/RyanShaw_B00634437_CW1#Nationlist"/>
        <hasTotalAveragePercentageChangeOfVote rdf:datatype="http://www.w3.org/2001/XMLSchema#decimal">-3.8</hasTotalAveragePercentageChangeOfVote>
        <hasTotalChangeInSeats rdf:datatype="http://www.w3.org/2001/XMLSchema#integer">1</hasTotalChangeInSeats>
        <hasTotalNumberOfCandidates rdf:datatype="http://www.w3.org/2001/XMLSchema#integer">2</hasTotalNumberOfCandidates>
        <hasTotalPercentageCandidateSuccessRate rdf:datatype="http://www.w3.org/2001/XMLSchema#integer">100</hasTotalPercentageCandidateSuccessRate>
        <hasTotalPercentageChangeInVote rdf:datatype="http://www.w3.org/2001/XMLSchema#decimal">-7.5</hasTotalPercentageChangeInVote>
        <hasTotalPercentageShareOfVote rdf:datatype="http://www.w3.org/2001/XMLSchema#decimal">24.7</hasTotalPercentageShareOfVote>
        <hasTotalSeatsWon rdf:datatype="http://www.w3.org/2001/XMLSchema#integer">2</hasTotalSeatsWon>
        <hasTotalVoteCount rdf:datatype="http://www.w3.org/2001/XMLSchema#integer">43944</hasTotalVoteCount>
    </owl:NamedIndividual>
    


    <!-- http://www.semanticweb.org/shawr/ontologies/2022/10/RyanShaw_B00634437_CW1#UlsterUnionist -->

    <owl:NamedIndividual rdf:about="http://www.semanticweb.org/shawr/ontologies/2022/10/RyanShaw_B00634437_CW1#UlsterUnionist">
        <rdf:type rdf:resource="http://www.semanticweb.org/shawr/ontologies/2022/10/RyanShaw_B00634437_CW1#Party"/>
        <hasAlignment rdf:resource="http://www.semanticweb.org/shawr/ontologies/2022/10/RyanShaw_B00634437_CW1#Unionist"/>
        <hasTotalAveragePercentageChangeOfVote rdf:datatype="http://www.w3.org/2001/XMLSchema#decimal">0.9</hasTotalAveragePercentageChangeOfVote>
        <hasTotalChangeInSeats rdf:datatype="http://www.w3.org/2001/XMLSchema#integer">0</hasTotalChangeInSeats>
        <hasTotalNumberOfCandidates rdf:datatype="http://www.w3.org/2001/XMLSchema#integer">2</hasTotalNumberOfCandidates>
        <hasTotalPercentageCandidateSuccessRate rdf:datatype="http://www.w3.org/2001/XMLSchema#integer">0</hasTotalPercentageCandidateSuccessRate>
        <hasTotalPercentageChangeInVote rdf:datatype="http://www.w3.org/2001/XMLSchema#decimal">1.8</hasTotalPercentageChangeInVote>
        <hasTotalPercentageShareOfVote rdf:datatype="http://www.w3.org/2001/XMLSchema#decimal">2.1</hasTotalPercentageShareOfVote>
        <hasTotalSeatsWon rdf:datatype="http://www.w3.org/2001/XMLSchema#integer">0</hasTotalSeatsWon>
        <hasTotalVoteCount rdf:datatype="http://www.w3.org/2001/XMLSchema#integer">3775</hasTotalVoteCount>
    </owl:NamedIndividual>
    


    <!-- http://www.semanticweb.org/shawr/ontologies/2022/10/RyanShaw_B00634437_CW1#Unionist -->

    <owl:NamedIndividual rdf:about="http://www.semanticweb.org/shawr/ontologies/2022/10/RyanShaw_B00634437_CW1#Unionist">
        <rdf:type rdf:resource="http://www.semanticweb.org/shawr/ontologies/2022/10/RyanShaw_B00634437_CW1#PoliticalAlignment"/>
    </owl:NamedIndividual>
    


    <!-- 
    ///////////////////////////////////////////////////////////////////////////////////////
    //
    // General axioms
    //
    ///////////////////////////////////////////////////////////////////////////////////////
     -->

    <rdf:Description>
        <rdf:type rdf:resource="http://www.w3.org/2002/07/owl#AllDisjointClasses"/>
        <owl:members rdf:parseType="Collection">
            <rdf:Description rdf:about="http://www.semanticweb.org/shawr/ontologies/2022/10/RyanShaw_B00634437_CW1#Candidate"/>
            <rdf:Description rdf:about="http://www.semanticweb.org/shawr/ontologies/2022/10/RyanShaw_B00634437_CW1#Constituency"/>
            <rdf:Description rdf:about="http://www.semanticweb.org/shawr/ontologies/2022/10/RyanShaw_B00634437_CW1#Party"/>
        </owl:members>
    </rdf:Description>
</rdf:RDF>



<!-- Generated by the OWL API (version 4.5.9.2019-02-01T07:24:44Z) https://github.com/owlcs/owlapi -->

